More changes to the parser; still problems with parsing the compiler

coq/theories/assembly/ASMToString.v
@@ -11,8 +11,7 @@ Notation "cst ::: s" :=
         | _ => fail "Left string is not constant"
         end) (at level 60, only parsing).
 
-(* This is named reg2str1, since when I named it reg2str, it reified forever, see example in AsmToStringDerivations.v *)
-Definition reg2str1 (r: reg) (str: string): string :=
+Definition reg2s (r: reg) (str: string): string :=
   match r with
   | RAX => "%rax" ++ str
   | RDI => "%rdi" ++ str
@@ -42,70 +41,70 @@ Fixpoint clean (cs: string) (acc: string): string :=
       res
   end.
 
-Definition inst2str_const (r: reg) (imm: word64) (str: string): string :=
-  "movq $" ++ N2str (Z.to_N (word.unsigned imm)) (", " ++ reg2str1 r str).
+Definition i2s_con (r: reg) (imm: word64) (str: string): string :=
+  "movq $" ++ N2str (Z.to_N (word.unsigned imm)) (", " ++ reg2s r str).
 
-Definition inst2str_mov (dst: reg) (src: reg) (str: string): string :=
-  "movq " ++ reg2str1 src (", " ++ reg2str1 dst str).
+Definition i2s_mov (dst: reg) (src: reg) (str: string): string :=
+  "movq " ++ reg2s src (", " ++ reg2s dst str).
 
-Definition inst2str_add (dst: reg) (src: reg) (str: string): string :=
-  "addq " ++ reg2str1 src (", " ++ reg2str1 dst str).
+Definition i2s_add (dst: reg) (src: reg) (str: string): string :=
+  "addq " ++ reg2s src (", " ++ reg2s dst str).
 
-Definition inst2str_sub (dst: reg) (src: reg) (str: string): string :=
-  "subq " ++ reg2str1 src (", " ++ reg2str1 dst str).
+Definition i2s_sub (dst: reg) (src: reg) (str: string): string :=
+  "subq " ++ reg2s src (", " ++ reg2s dst str).
 
-Definition inst2str_div (r: reg) (str: string): string :=
-  "divq " ++ reg2str1 r str.
+Definition i2s_div (r: reg) (str: string): string :=
+  "divq " ++ reg2s r str.
 
-Definition inst2str_jump (cond: cond) (n: nat) (str: string): string :=
+Definition i2s_jump (cond: cond) (n: nat) (str: string): string :=
   match cond with
     | Always => "jmp " ++ lab n str
     | Equal r1 r2 =>
-      "cmpq " ++ reg2str1 r2 (", " ++ reg2str1 r1 (" ; je " ++ lab n str))
+      "cmpq " ++ reg2s r2 (", " ++ reg2s r1 (" ; je " ++ lab n str))
     | Less r1 r2 =>
-      "cmpq " ++ reg2str1 r2 (", " ++ reg2str1 r1 (" ; jb " ++ lab n str))
+      "cmpq " ++ reg2s r2 (", " ++ reg2s r1 (" ; jb " ++ lab n str))
     end.
 
-Definition inst2str_call (n: nat) (str: string): string :=
+Definition i2s_call (n: nat) (str: string): string :=
   "call " ++ lab n str.
 
-Definition inst2str_ret (str: string): string :=
+Definition i2s_ret (str: string): string :=
   "ret" ++ str.
 
-Definition inst2str_pop (r: reg) (str: string): string :=
-  "popq " ++ reg2str1 r str.
+Definition i2s_pop (r: reg) (str: string): string :=
+  "popq " ++ reg2s r str.
 
-Definition inst2str_push (r: reg) (str: string): string :=
-  "pushq " ++ reg2str1 r str.
+Definition i2s_push (r: reg) (str: string): string :=
+  "pushq " ++ reg2s r str.
 
-Definition inst2str_load_rsp (r: reg) (n: nat) (str: string): string :=
-  "movq " ++ num2str (8 * n) ("(%rsp), " ++ reg2str1 r str).
+Definition i2s_lrsp (r: reg) (n: nat) (str: string): string :=
+  "movq " ++ num2str (8 * n) ("(%rsp), " ++ reg2s r str).
 
-Definition inst2str_store_rsp (r: reg) (n: nat) (str: string): string :=
-  "movq " ++ (reg2str1 r (", " ++ num2str (8 * n) ("(%rsp) " ++ str))).
+Definition i2s_srsp (r: reg) (n: nat) (str: string): string :=
+  "movq " ++ (reg2s r (", " ++ num2str (8 * n) ("(%rsp) " ++ str))).
 
-Definition inst2str_add_rsp (n: nat) (str: string): string :=
+Definition i2s_arsp (n: nat) (str: string): string :=
   "addq $" ++ num2str (8 * n) (", %rsp" ++ str).
 
-Definition inst2str_sub_rsp (n: nat) (str: string): string :=
+Definition i2s_surs (n: nat) (str: string): string :=
   "subq $" ++ num2str (8 * n) (", %rsp" ++ str).
 
-Definition inst2str_store (src: reg) (a: reg) (w: word4) (str: string): string :=
-  "movq " ++ reg2str1 src (", " ++ N2str (Z.to_N (word.unsigned w)) ("(" ++ reg2str1 a (")" ++ str))).
+Definition i2s_stor (src: reg) (a: reg) (w: word4) (str: string): string :=
+  "movq " ++ reg2s src (", " ++ N2str (Z.to_N (word.unsigned w)) ("(" ++ reg2s a (")" ++ str))).
 
-Definition inst2str_load (dst: reg) (a: reg) (w: word4) (str: string): string :=
-  "movq " ++ N2str (Z.to_N (word.unsigned w)) ("(" ++ reg2str1 a ("), " ++ reg2str1 dst str)).
+Definition i2s_load (dst: reg) (a: reg) (w: word4) (str: string): string :=
+  "movq " ++ N2str (Z.to_N (word.unsigned w)) ("(" ++ reg2s a ("), " ++ reg2s dst str)).
 
-Definition inst2str_getchar1 (str: string): string :=
+Definition i2s_gch (str: string): string :=
   "movq stdin(%rip), %rdi ; call _IO_getc@PLT" ++ str.
 
-Definition inst2str_putchar (str: string): string :=
+Definition i2s_pch (str: string): string :=
   "movq stdout(%rip), %rsi ; call _IO_putc@PLT" ++ str.
 
-Definition inst2str_exit (str: string): string :=
+Definition i2s_exit (str: string): string :=
   "call exit@PLT" ++ str.
 
-Definition inst2str_comment (c: string) (str: string): string :=
+Definition i2s_comm (c: string) (str: string): string :=
   "
   
   	/* " ++ clean c (" */" ++ str).
@@ -113,79 +112,79 @@ Definition inst2str_comment (c: string) (str: string): string :=
 Definition inst2str (i: instr) (str: string): string :=
   match i with
   | Const r imm =>
-    let/d res := inst2str_const r imm str in
+    let/d res := i2s_con r imm str in
     res
   | Mov dst src =>
-    let/d res := inst2str_mov dst src str in
+    let/d res := i2s_mov dst src str in
     res
   | ASMSyntax.Add dst src =>
-    let/d res := inst2str_add dst src str in
+    let/d res := i2s_add dst src str in
     res
   | Sub dst src =>
-    let/d res := inst2str_sub dst src str in
+    let/d res := i2s_sub dst src str in
     res
   | Div r =>
-    let/d res := inst2str_div r str in
+    let/d res := i2s_div r str in
     res
   | Jump cond n =>
-    inst2str_jump cond n str
+    i2s_jump cond n str
   | Call n =>
-    let/d res := inst2str_call n str in
+    let/d res := i2s_call n str in
     res
   | Ret =>
-    let/d res := inst2str_ret str in
+    let/d res := i2s_ret str in
     res
   | Pop r =>
-    let/d res := inst2str_pop r str in
+    let/d res := i2s_pop r str in
     res
   | Push r =>
-    let/d res := inst2str_push r str in
+    let/d res := i2s_push r str in
     res
   | Load_RSP r n =>
-    let/d res := inst2str_load_rsp r n str in
+    let/d res := i2s_lrsp r n str in
     res
   | StoreRSP r n =>
-    let/d res := inst2str_store_rsp r n str in
+    let/d res := i2s_srsp r n str in
     res
   | Add_RSP n =>
-    let/d res := inst2str_add_rsp n str in
+    let/d res := i2s_arsp n str in
     res
   | Sub_RSP n =>
-    let/d res := inst2str_sub_rsp n str in
+    let/d res := i2s_surs n str in
     res
   | Store src a w =>
-    let/d res := inst2str_store src a w str in
+    let/d res := i2s_stor src a w str in
     res
   | Load dst a w =>
-    let/d res := inst2str_load dst a w str in
+    let/d res := i2s_load dst a w str in
     res
   | GetChar =>
-    let/d res := inst2str_getchar1 str in
+    let/d res := i2s_gch str in
     res
   | PutChar =>
-    let/d res := inst2str_putchar str in
+    let/d res := i2s_pch str in
     res
   | Exit =>
-    let/d res := inst2str_exit str in
+    let/d res := i2s_exit str in
     res
   | Comment c =>
-    let/d res := inst2str_comment c str in
+    let/d res := i2s_comm c str in
     res
   end.
 
 
-Fixpoint instrs2str (n: nat) (is: asm): string :=
+Fixpoint is2str (n: nat) (is: asm): string :=
   match is with
   | [] => EmptyString
   | i :: is =>
-    lab n (String ":" (String "009" (inst2str i (String "010" (instrs2str (n+1) is)))))
+    lab n (String ":" (String "009" (inst2str i (String "010" (is2str (n+1) is)))))
   end.
 
-Fixpoint concat_strings (ss: list string): string :=
+Fixpoint ccat_str (ss: list string): string :=
   match ss with
   | [] => EmptyString
   | s :: ss =>
-    s ++ concat_strings ss
+    s ++ ccat_str ss
   end.
 
 Definition asm2str1 :=
@@ -216,18 +215,18 @@ Definition asm2str8 :=
 Definition asm2str9 :=
   "main:
   ".
-Definition asm2str10 :=
+Definition asm2str0 :=
   "	subq $8, %rsp        /* 16-byte align %rsp */
   ".
-Definition asm2str11 :=
+Definition asm2stra :=
   "	movabs $heapS, %r14  /* r14 := heap start  */
   ".
-Definition asm2str12 :=
+Definition asm2strb :=
   "	movabs $heapE, %r15  /* r15 := heap end    */
   
   ".
 
-Definition asm2str (is: asm): string := concat_strings
+Definition asm2str (is: asm): string := ccat_str
   [asm2str1;
     asm2str2;
     asm2str3;
@@ -237,8 +236,8 @@ Definition asm2str (is: asm): string := concat_strings
     asm2str7;
     asm2str8;
     asm2str9;
-    asm2str10;
-    asm2str11;
-    asm2str12
+    asm2str0;
+    asm2stra;
+    asm2strb
     ]%string
-  ++ instrs2str 0 is.
+  ++ is2str 0 is.
