coq/theories/commons/CompilerUtils.v
@@ -5,62 +5,62 @@ Require Import coqutil.Word.Interface.
 Require Import coqutil.Word.Properties.
 From impboot Require Import commons.ProofUtils.
 
-Fixpoint mul_nat (a b: nat): nat :=
+Fixpoint mulnat (a b: nat): nat :=
   match b with
   | 0%nat => 0%nat
-  | S b' => a + mul_nat a b'
+  | S b' => a + mulnat a b'
   end.
 
-Definition nat_modulo (n1 n2: nat): nat :=
+Definition nat_mod (n1 n2: nat): nat :=
   match n2 with
   | 0%nat => 0
   | S _ => n1  - (n2 * (n1 / n2))
   end.
 
-Definition nat_modulo_10 (n: nat): nat :=
+Definition natmod10 (n: nat): nat :=
   n - (10 * (n / 10)).
 
-Lemma nat_modulo_10_spec: forall n,
-  nat_modulo_10 n = nat_modulo n 10.
+Lemma natmod10_spec: forall n,
+  natmod10 n = nat_mod n 10.
 Proof. reflexivity. Qed.
 
-Lemma mul_N_f_oblig:
+Lemma mulN_f_oblig:
   forall (b_min_1 b: N) (NE: b <> 0%N) (BMIN1EQ: b_min_1 = (b - 1)%N), (b_min_1 < b)%N.
 Proof.
   intros; subst.
   apply N.sub_lt; lia.
 Qed.
 
-Fixpoint mul_N_f (a b: N) (fuel: nat): N :=
+Fixpoint mulN_f (a b: N) (fuel: nat): N :=
   match fuel with
   | 0%nat => 0%N
   | S fuel =>
     match b with
     | 0%N => 0%N
-    | _ => a + mul_N_f a (b - 1) fuel
+    | _ => a + mulN_f a (b - 1) fuel
     end
   end.
 
-Definition mul_N_10 (a: N): N :=
+Definition mulN_10 (a: N): N :=
   (let/d a2 := a + a in
   let/d a4 := a2 + a2 in
   let/d a8 := a4 + a4 in
   let/d a10 := a8 + a2 in
   a10)%N.
 
-Lemma mul_N_10_spec_r: forall a,
-  mul_N_10 a = (a * 10)%N.
+Lemma mulN_10_spec_r: forall a,
+  mulN_10 a = (a * 10)%N.
 Proof.
-  intros; unfold mul_N_10, dlet; simpl; lia.
+  intros; unfold mulN_10, dlet; simpl; lia.
 Qed.
 
-Lemma mul_N_10_spec_l: forall a,
-  mul_N_10 a = (10 * a)%N.
+Lemma mulN_10_spec_l: forall a,
+  mulN_10 a = (10 * a)%N.
 Proof.
-  intros; unfold mul_N_10, dlet; simpl; destruct a; simpl; lia.
+  intros; unfold mulN_10, dlet; simpl; destruct a; simpl; lia.
 Qed.
 
-Definition mul_N_256 (a: N): N :=
+Definition mulN_256 (a: N): N :=
   (let/d a2 := a + a in
   let/d a4 := a2 + a2 in
   let/d a8 := a4 + a4 in
@@ -71,62 +71,62 @@ Definition mul_N_256 (a: N): N :=
   let/d a256 := a128 + a128 in
   a256)%N.
 
-Lemma mul_N_256_spec_r: forall a,
-  mul_N_256 a = (a * 256)%N.
+Lemma mulN_256_spec_r: forall a,
+  mulN_256 a = (a * 256)%N.
 Proof.
-  intros; unfold mul_N_256, dlet; simpl; lia.
+  intros; unfold mulN_256, dlet; simpl; lia.
 Qed.
 
-Lemma mul_N_256_spec_l: forall a,
-  mul_N_256 a = (256 * a)%N.
+Lemma mulN_256_spec_l: forall a,
+  mulN_256 a = (256 * a)%N.
 Proof.
-  intros; unfold mul_N_256, dlet; simpl; destruct a; simpl; lia.
+  intros; unfold mulN_256, dlet; simpl; destruct a; simpl; lia.
 Qed.
 
-Definition mul_nat_8 (a: nat): nat :=
+Definition mulnat_8 (a: nat): nat :=
   let/d a2 := a + a in
   let/d a4 := a2 + a2 in
   let/d a8 := a4 + a4 in
   a8.
 
-Lemma mul_nat_8_spec_r: forall a,
-  mul_nat_8 a = (a * 8)%nat.
+Lemma mulnat_8_spec_r: forall a,
+  mulnat_8 a = (a * 8)%nat.
 Proof.
-  intros; unfold mul_nat_8, dlet; simpl; lia.
+  intros; unfold mulnat_8, dlet; simpl; lia.
 Qed.
 
-Lemma mul_nat_8_spec_l: forall a,
-  mul_nat_8 a = (8 * a)%nat.
+Lemma mulnat_8_spec_l: forall a,
+  mulnat_8 a = (8 * a)%nat.
 Proof.
-  intros; unfold mul_nat_8, dlet; simpl; lia.
+  intros; unfold mulnat_8, dlet; simpl; lia.
 Qed.
 
-Definition mul_nat_10 (a: nat): nat :=
+Definition mulnat10 (a: nat): nat :=
   let/d a2 := a + a in
   let/d a4 := a2 + a2 in
   let/d a8 := a4 + a4 in
   let/d a10 := a8 + a2 in
   a10.
 
-Lemma mul_nat_10_spec_r: forall a,
-  mul_nat_10 a = (a * 10)%nat.
+Lemma mulnat10_spec_r: forall a,
+  mulnat10 a = (a * 10)%nat.
 Proof.
-  intros; unfold mul_nat_10, dlet; simpl; lia.
+  intros; unfold mulnat10, dlet; simpl; lia.
 Qed.
 
-Lemma mul_nat_10_spec_l: forall a,
-  mul_nat_10 a = (10 * a)%nat.
+Lemma mulnat10_spec_l: forall a,
+  mulnat10 a = (10 * a)%nat.
 Proof.
-  intros; unfold mul_nat_10, dlet; simpl; lia.
+  intros; unfold mulnat10, dlet; simpl; lia.
 Qed.
 
-Definition mul_N (a b: N): N :=
-  mul_N_f a b (1 + N.to_nat b).
+Definition mulN (a b: N): N :=
+  mulN_f a b (1 + N.to_nat b).
 
-Lemma mul_N_f_terminates: forall (fuel: nat) (a b: N) ,
+Lemma mulN_f_terminates: forall (fuel: nat) (a b: N) ,
   a <> 0%N -> b <> 0%N ->
   fuel = S (N.to_nat b) ->
-  mul_N_f a b fuel <> 0%N.
+  mulN_f a b fuel <> 0%N.
 Proof.
   intros fuel a b Ha Hb Hfuel.
   destruct fuel; [lia|].
@@ -135,9 +135,9 @@ Proof.
   lia.
 Qed.
 
-Lemma mul_N_f_spec: forall (fuel: nat) (a b: N),
+Lemma mulN_f_spec: forall (fuel: nat) (a b: N),
   fuel = S (N.to_nat b) ->
-  mul_N_f a b fuel = (a * b)%N.
+  mulN_f a b fuel = (a * b)%N.
 Proof.
   induction fuel; intros.
   - lia.
@@ -145,7 +145,7 @@ Proof.
     + simpl. lia.
     + unfold dlet; simpl.
       match goal with
-      | |- context [mul_N_f ?a ?x ?f] =>
+      | |- context [mulN_f ?a ?x ?f] =>
         replace x with (N.pos p - 1)%N by reflexivity
       end.
       rewrite IHfuel.
@@ -155,17 +155,17 @@ Proof.
       * rewrite Nnat.N2Nat.inj_sub. simpl in *. lia.
 Qed.
 
-Theorem mul_N_spec: forall (a b: N),
-  mul_N a b = (a * b)%N.
+Theorem mulN_spec: forall (a b: N),
+  mulN a b = (a * b)%N.
 Proof.
   intros.
-  unfold mul_N, dlet.
-  apply mul_N_f_spec.
+  unfold mulN, dlet.
+  apply mulN_f_spec.
   lia.
 Qed.
 
-Theorem mul_nat_spec: forall (a b: nat),
-  mul_nat a b = a * b.
+Theorem mulnat_spec: forall (a b: nat),
+  mulnat a b = a * b.
 Proof.
   induction b; intros; simpl; unfold dlet; simpl.
   - lia.
@@ -179,25 +179,25 @@ Definition N_modulo (n1 n2: N): N :=
   | _ => n1  - (n2 * (n1 / n2))
   end.
 
-Definition N_modulo_10 (n: N): N :=
+Definition Nmod_10 (n: N): N :=
   n - (10 * (n / 10)).
 
-Lemma N_modulo_10_spec: forall n,
-  N_modulo_10 n = N_modulo n 10.
+Lemma Nmod_10_spec: forall n,
+  Nmod_10 n = N_modulo n 10.
 Proof. reflexivity. Qed.
 
-Definition N_modulo_256 (n: N): N :=
+Definition Nmod_256 (n: N): N :=
   n - (256 * (n / 256)).
 
-Lemma N_modulo_256_spec: forall n,
-  N_modulo_256 n = N_modulo n 256.
+Lemma Nmod_256_spec: forall n,
+  Nmod_256 n = N_modulo n 256.
 Proof. reflexivity. Qed.
 
-Theorem nat_modulo_le: forall (n m: nat),
-  nat_modulo n m <= m.
+Theorem nat_mod_le: forall (n m: nat),
+  nat_mod n m <= m.
 Proof.
   intros.
-  unfold nat_modulo, dlet.
+  unfold nat_mod, dlet.
   destruct m; try lia.
   rewrite <- Nat.Div0.mod_eq.
   specialize Nat.mod_upper_bound with (a := n) (b := S m) as ?.
@@ -228,21 +228,21 @@ Proof.
   eapply N.mod_lt; lia.
 Qed.
 
-Fixpoint num2str_f (n: nat) (fuel: nat) (str: string): string :=
+Fixpoint num2strf (n: nat) (fuel: nat) (str: string): string :=
   if (n <? 10)%nat then
-    let/d nd := nat_modulo n 10 in
+    let/d nd := nat_mod n 10 in
     let/d a:= ascii_of_nat (48 + nd) in
     String a str
   else match fuel with
   | 0 => ""
   | S fuel =>
-    let/d nd := nat_modulo n 10 in
+    let/d nd := nat_mod n 10 in
     let/d a := ascii_of_nat (48 + nd) in
-    num2str_f (n / 10) fuel (String a str)
+    num2strf (n / 10) fuel (String a str)
   end.
 
 Theorem num2str_terminates_str: forall (n1: nat) (n: nat) (str: string),
-  n <= n1 -> num2str_f n n1 str <> ""%string.
+  n <= n1 -> num2strf n n1 str <> ""%string.
 Proof.
   induction n1; intros; simpl; unfold dlet; simpl; [inversion H; simpl; congruence|].
   destruct (n <? 10)%nat; [congruence|].
@@ -253,7 +253,7 @@ Proof.
 Qed.
 
 Definition num2str (n: nat) (str: string): string :=
-  num2str_f n n str.
+  num2strf n n str.
 
 Theorem num2str_terminates: forall (n: nat) (str: string),
   num2str n str <> ""%string.
@@ -263,13 +263,13 @@ Qed.
 
 Fixpoint N2str_f (n: N) (fuel: nat) (str: string): string :=
   if (n <? 10)%N then
-    let/d nd := N_modulo_10 n in
+    let/d nd := Nmod_10 n in
     let/d a:= ascii_of_N (48 + nd) in
     String a str
   else match fuel with
   | 0 => ""
   | S fuel =>
-    let/d nd := N_modulo_10 n in
+    let/d nd := Nmod_10 n in
     let/d a := ascii_of_N (48 + nd) in
     N2str_f (n / 10) fuel (String a str)
   end.
@@ -307,26 +307,26 @@ Proof.
   destruct (n mod 10)%N eqn:?; rewrite ?N.eqb_eq, ?N.eqb_neq in *; subst; try lia.
 Qed.
 
-Fixpoint list_length {A: Type} (l: list A): nat :=
+Fixpoint list_len {A: Type} (l: list A): nat :=
   match l with
-  | x :: l => 1 + list_length l
+  | x :: l => 1 + list_len l
   | [] => 0
   end.
 
-Theorem list_length_spec: forall {A: Type} (l: list A),
-  list_length l = List.length l.
+Theorem list_len_spec: forall {A: Type} (l: list A),
+  list_len l = List.length l.
 Proof.
   induction l; simpl; unfold dlet; simpl; eauto.
 Qed.
 
-Fixpoint list_append {A: Type} (l1 l2: list A): list A :=
+Fixpoint list_app {A: Type} (l1 l2: list A): list A :=
   match l1 with
-  | x :: l1 => x :: list_append l1 l2
+  | x :: l1 => x :: list_app l1 l2
   | [] => l2
   end.
 
-Theorem list_append_spec: ∀ {A: Type} (l1 l2: list A),
-  list_append l1 l2 = l1 ++ l2.
+Theorem list_app_spec: ∀ {A: Type} (l1 l2: list A),
+  list_app l1 l2 = l1 ++ l2.
 Proof.
   induction l1; simpl; unfold dlet; simpl; eauto.
   intros; f_equal; eauto.
@@ -336,25 +336,25 @@ Fixpoint flatten {A: Type} (xs: app_list A): list A :=
   match xs with
   | List l => l
   | Append l1 l2 =>
-    list_append (flatten l1) (flatten l2)
+    list_app (flatten l1) (flatten l2)
   end.
 
-Fixpoint app_list_length {A: Type} (xs: app_list A): nat :=
+Fixpoint appl_len {A: Type} (xs: app_list A): nat :=
   match xs with
-  | List l => list_length l
+  | List l => list_len l
   | Append l1 l2 =>
-    app_list_length l1 + app_list_length l2
+    appl_len l1 + appl_len l2
   end.
 
-Fixpoint string_append (s1 s2: string): string :=
+Fixpoint str_app (s1 s2: string): string :=
   match s1 with
   | EmptyString => s2
   | String c s1 =>
-    String c (string_append s1 s2)
+    String c (str_app s1 s2)
   end.
 
-Lemma string_append_spec: forall s1 s2,
-  string_append s1 s2 = (s1 ++ s2)%string.
+Lemma str_app_spec: forall s1 s2,
+  str_app s1 s2 = (s1 ++ s2)%string.
 Proof.
   induction s1; intros; simpl; unfold dlet; simpl.
   - reflexivity.
@@ -364,7 +364,7 @@ Qed.
 
 Open Scope string_scope.
 
-Fixpoint N2ascii_f (n: N) (fuel: nat): option string :=
+Fixpoint N2asciif (n: N) (fuel: nat): option string :=
   if (n =? 0)%N then None else
   let/d k := N_modulo n 256 in
   if (k <? N_of_ascii "*"%char)%N then None else
@@ -374,15 +374,15 @@ Fixpoint N2ascii_f (n: N) (fuel: nat): option string :=
   match fuel with
   | 0%nat => Some EmptyString
   | S fuel =>
-    let/d r := N2ascii_f (n / 256) fuel in
+    let/d r := N2asciif (n / 256) fuel in
     match r return option string with
     | None => None
     | Some s => Some (s ++ String (ascii_of_N k) EmptyString)
     end
   end.
 
-Theorem N2ascii_f_terminates: forall (n1: nat) (n: N),
-  (n <= ((N.of_nat n1 * 256) - 1))%N -> N2ascii_f n n1 <> Some EmptyString.
+Theorem N2asciif_terminates: forall (n1: nat) (n: N),
+  (n <= ((N.of_nat n1 * 256) - 1))%N -> N2asciif n n1 <> Some EmptyString.
 Proof.
   Opaque N.add N.div N_modulo N_of_ascii.
   induction n1; intros; simpl; unfold dlet; simpl.
@@ -392,25 +392,25 @@ Proof.
   destruct (_ <? k)%N eqn:?; try congruence.
   destruct (_ =? _)%N eqn:?; try congruence.
   destruct (n <? _)%N eqn:?; [congruence|]; rewrite N.ltb_ge in *.
-  destruct N2ascii_f; try congruence.
+  destruct N2asciif; try congruence.
   destruct s; simpl; try congruence.
 Qed.
 Transparent N.add N.div N_modulo N_of_ascii.
 
 Definition N2ascii (n: N): option string :=
-  N2ascii_f n (N.to_nat (n / 256 + 1)).
+  N2asciif n (N.to_nat (n / 256 + 1)).
 
 Theorem N2ascii_terminates: forall (n: N),
   N2ascii n <> Some EmptyString.
 Proof.
-  intros; eapply N2ascii_f_terminates; rewrite Nnat.N2Nat.id.
+  intros; eapply N2asciif_terminates; rewrite Nnat.N2Nat.id.
   rewrite (N.div_mod n 256) at 1 by discriminate.
   rewrite N.mul_comm, N.mul_add_distr_r, N.mul_1_l.
   assert (n mod 256 < 256)%N by (eapply N.mod_lt; lia).
   destruct (n mod 256)%N eqn:?; rewrite ?N.eqb_eq, ?N.eqb_neq in *; subst; try lia.
 Qed.
 
-Definition N2ascii_default (n: N): string :=
+Definition N2asciid (n: N): string :=
   let/d s := N2ascii n in
   match s return string with
   | None => ""
