coq/theories/imp2asm/CompilerProofs.v
@@ -1,10 +1,96 @@
-From impboot.utils Require Import Core.
+From impboot.utils Require Import Core Llist.
 From impboot.imp2asm Require Import Compiler.
 From impboot.parsing Require Import Parser.
 From impboot.imperative Require Import Printing.
 From impboot.bootstrapping Require Import Bootstrapping.
+From impboot.assembly Require Import ASMSemantics.
+From impboot.imperative Require Import ImpSyntax.
+From impboot.derivations Require Import CompilerDerivations.
+From impboot.imp2asm Require Import ImpToASMCodegenProofs.
+From impboot.fp2imp Require Import FpToImpCodegenProof.
+
+(* forall input prog output1 output2,
+    prog_terminates input prog fuel output1 sd /\
+    asm_terminates input (codegen prog) sd output2 ->
+      output1 = output2. *)
+
+(* 
+Theorem compiler_asm_correct:
+  ∀input output.
+    (input, compiler_asm) asm_terminates output ⇒
+    output = compiler input
+Proof
+  metis_tac [compiler_asm_def,codegen_terminates,compiler_prog_correct]
+QED
+
+Theorem compiler_compiler_str:
+  compiler compiler_str = compiler_asm_str
+Proof
+  fs [compiler_str_def,codegenTheory.compiler_def,
+      parser_lexer_prog2str,compiler_asm_str_def,compiler_asm_def]
+QED
+
+Theorem compiler_asm_bootstrap:
+  (compiler_str, compiler_asm) asm_terminates output ⇒
+  output = compiler_asm_str
+Proof
+  metis_tac [compiler_asm_correct,compiler_compiler_str]
+QED
+*)
+
+Theorem compiler_correct: forall input output sd,
+  asm_terminates (Llist.of_list input) compiler_program_asm sd output ->
+  output = compiler input.
+Proof.
+  intros * Hasm_terminates.
+  specialize (compiler_program_thm input) as Hfp_compiler_thm.
+  specialize compiler_program_imp_exists as [compiler_imp Hcompiler_program_imp]; subst.
+  unfold compiler_program_imp in *.
+  eapply to_imp_thm in Hfp_compiler_thm; eauto.
+  unfold ImpSemantics.imp_weak_termination in *; cleanup.
+  eapply codegen_terminates with (output2 := compiler input).
+Admitted.
+
+Set Printing Width 200.
+
+(* Time Eval lazy in match compiler_program_imp with
+  | None => ""
+  | Some compiler_imp =>
+    (imp2str compiler_imp)
+  end. *)
+
+Time Eval lazy in match compiler_program_imp with
+  | None => Program []
+  | Some compiler_imp =>
+    compiler_imp
+  end.
+
+Time Eval lazy in match compiler_program_imp with
+  | None => Program []
+  | Some compiler_imp =>
+    str2imp (list_ascii_of_string (imp2str compiler_imp))
+  end.
+
+Definition option_to_list {A} (o : option A) : list A :=
+  match o with
+  | None => []
+  | Some x => [x]
+  end.
 
 Theorem print_parser_compiler_correct:
+  match compiler_program_imp with
+  | None => False
+  | Some (ImpSyntax.Program fs) =>
+    let compiler_imp := ImpSyntax.Program (option_to_list (nth_error fs 0)) in
+    compiler_imp = str2imp (list_ascii_of_string (imp2str compiler_imp))
+    (* imp2str compiler_imp = "" *)
+  end.
+Proof.
+  lazy.
+  reflexivity.
+Qed.
+
+(* Theorem print_parser_compiler_correct:
   match compiler_program_imp with
   | None => False
   | Some compiler_imp =>
@@ -12,4 +98,4 @@ Theorem print_parser_compiler_correct:
   end.
 Proof.
   lazy; reflexivity.
-Qed.
+Qed. *)
