coq/theories/imp2asm/ImpToASMCodegen.v
@@ -110,23 +110,6 @@ Fixpoint index_of (vs: v_stack) (n: name) (k: nat): nat :=
 Theorem index_of_equation: ltac2:(unfold_fix_type '@index_of).
 Proof. unfold_fix_proof '@index_of. Qed.
 
-Fixpoint index_of_opt (vs: v_stack) (n: name) (k: nat): option nat :=
-  match vs with
-  | nil => None
-  | x :: vs =>
-    match x with
-    | None =>
-      index_of_opt vs n (k + 1)
-    | Some v =>
-      if N.eqb v n then
-        Some k
-      else
-        index_of_opt vs n (k + 1)
-    end
-  end.
-Theorem index_of_opt_equation: ltac2:(unfold_fix_type '@index_of_opt).
-Proof. unfold_fix_proof '@index_of_opt. Qed.
-
 (* lookup variable with name `n`, based on stack `vs` *)
 Definition c_var (n: name) (l: nat) (vs: v_stack): asm_appl * nat :=
   let/d k := index_of vs n 0 in
@@ -195,34 +178,34 @@ Fixpoint c_exp (e: exp) (l: nat) (vs: v_stack): asm_appl * nat :=
     let/d '(asm1, l1) := c_exp e1 l vs in
     let/d vs1 := None :: vs in
     let/d '(asm2, l2) := c_exp e2 l1 vs1 in
-    let/d c_add_asm := c_add in
-    let/d c_add_len := app_list_length c_add_asm in
-    let/d l3 := l2 + c_add_len in
-    (asm1 +++ asm2 +++ c_add_asm, l3)
+    let/d aasm := c_add in
+    let/d aasmlen := appl_len aasm in
+    let/d l3 := l2 + aasmlen in
+    (asm1 +++ asm2 +++ aasm, l3)
   | Sub e1 e2 =>
     let/d '(asm1, l1) := c_exp e1 l vs in
     let/d vs1 := None :: vs in
     let/d '(asm2, l2) := c_exp e2 l1 vs1 in
-    let/d c_sub_asm := c_sub in
-    let/d c_sub_len := app_list_length c_sub_asm in
-    let/d l3 := l2 + c_sub_len in
-    (asm1 +++ asm2 +++ c_sub_asm, l3)
+    let/d sasm := c_sub in
+    let/d sasmlen := appl_len sasm in
+    let/d l3 := l2 + sasmlen in
+    (asm1 +++ asm2 +++ sasm, l3)
   | Div e1 e2 =>
     let/d '(asm1, l1) := c_exp e1 l vs in
     let/d vs1 := None :: vs in
     let/d '(asm2, l2) := c_exp e2 l1 vs1 in
-    let/d cdiv := c_div in
-    let/d c_div_len := app_list_length cdiv in
-    let/d l3 := l2 + c_div_len in
-    (asm1 +++ asm2 +++ cdiv, l3)
+    let/d dasm := c_div in
+    let/d dasmlen := appl_len dasm in
+    let/d l3 := l2 + dasmlen in
+    (asm1 +++ asm2 +++ dasm, l3)
   | Read e1 e2 =>
     let/d '(asm1, l1) := c_exp e1 l vs in
     let/d vs1 := None :: vs in
     let/d '(asm2, l2) := c_exp e2 l1 vs1 in
-    let/d cload := c_load in
-    let/d c_load_len := app_list_length cload in
-    let/d l3 := l2 + c_load_len in
-    (asm1 +++ asm2 +++ cload, l3)
+    let/d lasm := c_load in
+    let/d lasmlen := appl_len lasm in
+    let/d l3 := l2 + lasmlen in
+    (asm1 +++ asm2 +++ lasm, l3)
   end.
 Theorem c_exp_equation: ltac2:(unfold_fix_type '@c_exp).
 Proof. unfold_fix_proof '@c_exp. Qed.
@@ -251,7 +234,7 @@ Definition c_cmp (c: cmp) : cond :=
     ASMSyntax.Equal RDI RBX
   end.
 
-Fixpoint c_test_jump (t: test) (pos_label: nat) (neg_label: nat)
+Fixpoint c_test (t: test) (pos_lbl: nat) (neg_lbl: nat)
   (l: nat) (vs: v_stack): asm_appl * nat :=
   match t with
   | Test c e1 e2 =>
@@ -259,29 +242,29 @@ Fixpoint c_test_jump (t: test) (pos_label: nat) (neg_label: nat)
     let/d vs1 := None :: vs in
     let/d '(asm2, l2) := c_exp e2 l1 vs1 in
     let/d cmp_cond := c_cmp c in
-    let/d c_cmp_asm := List [Mov RBX RAX; Pop RDI; Pop RAX; ASMSyntax.Jump cmp_cond pos_label; ASMSyntax.Jump Always neg_label] in
-    let/d c_cmp_len := app_list_length c_cmp_asm in
-    let/d l3 := l2 + c_cmp_len in
-    (asm1 +++ asm2 +++ c_cmp_asm, l3)
+    let/d cmp_asm := List [Mov RBX RAX; Pop RDI; Pop RAX; ASMSyntax.Jump cmp_cond pos_lbl; ASMSyntax.Jump Always neg_lbl] in
+    let/d cmp_len := appl_len cmp_asm in
+    let/d l3 := l2 + cmp_len in
+    (asm1 +++ asm2 +++ cmp_asm, l3)
   | And t1 t2 =>
     let/d l1_label := l + 1 in
     let/d l2_label := l + 2 in
-    let/d '(asm1, l1) := c_test_jump t1 l1_label neg_label l2_label vs in
-    let/d '(asm2, l2) := c_test_jump t2 pos_label neg_label l1 vs in
+    let/d '(asm1, l1) := c_test t1 l1_label neg_lbl l2_label vs in
+    let/d '(asm2, l2) := c_test t2 pos_lbl neg_lbl l1 vs in
     let/d asm0 := List [ASMSyntax.Jump Always l2_label; ASMSyntax.Jump Always l1] in
     (asm0 +++ asm1 +++ asm2, l2)
   | Or t1 t2 =>
     let/d l1_label := l + 1 in
     let/d l2_label := l + 2 in
-    let/d '(asm1, l1) := c_test_jump t1 pos_label l1_label l2_label vs in
-    let/d '(asm2, l2) := c_test_jump t2 pos_label neg_label l1 vs in
+    let/d '(asm1, l1) := c_test t1 pos_lbl l1_label l2_label vs in
+    let/d '(asm2, l2) := c_test t2 pos_lbl neg_lbl l1 vs in
     let/d asm0 := List [ASMSyntax.Jump Always l2_label; ASMSyntax.Jump Always l1] in
     (asm0 +++ asm1 +++ asm2, l2)
   | Not t' =>
-    c_test_jump t' neg_label pos_label l vs
+    c_test t' neg_lbl pos_lbl l vs
   end.
-Theorem c_test_jump_equation: ltac2:(unfold_fix_type '@c_test_jump).
-Proof. unfold_fix_proof '@c_test_jump. Qed.
+Theorem c_test_equation: ltac2:(unfold_fix_type '@c_test).
+Proof. unfold_fix_proof '@c_test. Qed.
 
 (* Looks up a function name in a list of function addresses *)
 Fixpoint lookup (fs: f_lookup) (n: N): nat :=
@@ -298,13 +281,13 @@ Proof. unfold_fix_proof '@lookup. Qed.
 
 (* Drop the current stack frame - elements corresponding to `vs` *)
 Definition make_ret (vs: v_stack) (l: nat): asm_appl * nat :=
-  let/d vs_len := list_length vs in
+  let/d vs_len := list_len vs in
   (List [Add_RSP vs_len; Ret], l + 2).
 
 (* Store the variables from the stack in the registers, so that they can be
 passed to the function call *)
 Definition c_pops (xs: list exp) (vs: v_stack): asm_appl :=
-  let/d k := list_length xs in
+  let/d k := list_len xs in
   if k =? 0 then 
     List [Push RAX]
   else if k =? 1 then 
@@ -327,26 +310,26 @@ so the actual stack size is odd then)
 *)
 
 (** Builds a stack representation for parameters of a function *)
-Fixpoint call_v_stack (xs: list name) (acc: v_stack): v_stack :=
+Fixpoint call_vs (xs: list name) (acc: v_stack): v_stack :=
   match xs with
   | [] => acc
   | x :: xs' =>
-    let/d some_x := Some x in
-    let/d x_acc := some_x :: acc in
-    call_v_stack xs' x_acc
+    let/d x_acc := Some x :: acc in
+    call_vs xs' x_acc
   end.
-Theorem call_v_stack_equation: ltac2:(unfold_fix_type '@call_v_stack).
-Proof. unfold_fix_proof '@call_v_stack. Qed.
+Theorem call_vs_equation: ltac2:(unfold_fix_type '@call_vs).
+Proof. unfold_fix_proof '@call_vs. Qed.
 
-Definition c_pushes_vs (v_names: list name): list (option name) :=
-  let/d len := list_length v_names in
+Definition push_vs (v_names: list name): list (option name) :=
+  let/d len := list_len v_names in
   if len =? 0 then [None]
   else
-    call_v_stack v_names (@nil (option name)).
+    call_vs v_names (@nil (option name)).
+
 (** Push a list of variables onto the stack *)
 Definition c_pushes (v_names: list name) (l: nat): (asm_appl * v_stack * nat) :=
-  let/d k := list_length v_names in
-  let/d e := c_pushes_vs v_names in
+  let/d k := list_len v_names in
+  let/d e := push_vs v_names in
   if k =? 0 then 
     ((List [], e), l)
   else if k =? 1 then 
@@ -363,9 +346,9 @@ Definition c_pushes (v_names: list name) (l: nat): (asm_appl * v_stack * nat) :=
 (* Call the given function, passing the arguments in registers*)
 Definition c_call (vs: v_stack) (target: nat) (xs: list exp) (l: nat): asm_appl * nat :=
   let/d asm_pops := c_pops xs vs in
-  let/d asm_combined := asm_pops +++ List [ASMSyntax.Call target] in
-  let/d total_len := app_list_length asm_pops + 1 in
-  (asm_combined, l + total_len).
+  let/d asm_cmb := asm_pops +++ List [ASMSyntax.Call target] in
+  let/d len := appl_len asm_pops + 1 in
+  (asm_cmb, l + len).
 
 Fixpoint c_cmd (c: cmd) (l: nat) (fs: f_lookup) (vs: v_stack): (asm_appl * nat) :=
   match c with
@@ -383,33 +366,33 @@ Fixpoint c_cmd (c: cmd) (l: nat) (fs: f_lookup) (vs: v_stack): (asm_appl * nat) 
     let/d '(asm1, l1) := c_exp a l vs in
     let/d '(asm2, l2) := c_exp e l1 (None :: vs) in
     let/d '(asm3, l3) := c_exp e' l2 (None :: None :: vs) in
-    let/d asm4_len := app_list_length c_store in
+    let/d asm4_len := appl_len c_store in
     (asm1 +++ asm2 +++ asm3 +++ c_store, l3 + asm4_len)
   | If t c1 c2 =>
     let/d l1_label := l + 1 in
     let/d l2_label := l + 2 in
     let/d l3_label := l + 3 in
-    let/d '(asm1, l1) := c_test_jump t l1_label l2_label l3_label vs in
+    let/d '(asm1, l1) := c_test t l1_label l2_label l3_label vs in
     let/d '(asm2, l2) := c_cmd c1 l1 fs vs in
     let/d '(asm3, l3) := c_cmd c2 (l2 + 1) fs vs in
-    let/d asm_combined := List [ASMSyntax.Jump Always l3_label;
+    let/d asm_cmb := List [ASMSyntax.Jump Always l3_label;
                           ASMSyntax.Jump Always l1;
                           ASMSyntax.Jump Always (l2 + 1)] +++ 
                           asm1 +++ asm2 +++ 
                           List [ASMSyntax.Jump Always l3] +++ asm3 in
-    (asm_combined, l3)
+    (asm_cmb, l3)
   | While tst body =>
     let/d l1_label := l + 1 in
     let/d l2_label := l + 2 in
     let/d l3_label := l + 3 in
-    let/d '(asm1, l1) := c_test_jump tst l1_label l2_label l3_label vs in
+    let/d '(asm1, l1) := c_test tst l1_label l2_label l3_label vs in
     let/d '(asm2, l2) := c_cmd body l1 fs vs in
-    let/d asm_combined := List [ASMSyntax.Jump Always l3_label] +++ 
+    let/d asm_cmb := List [ASMSyntax.Jump Always l3_label] +++ 
                           List [ASMSyntax.Jump Always l1] +++ 
                           List [ASMSyntax.Jump Always (l2 + 1)] +++ 
                           asm1 +++ asm2 +++ 
                           List [ASMSyntax.Jump Always l] in
-    (asm_combined, l2 + 1)
+    (asm_cmb, l2 + 1)
   | Call n f es =>
     let/d '(asms, l1) := c_exps es l vs in
     let/d '(asm1, l2) := c_call vs (lookup fs f) es l1 in
@@ -421,7 +404,7 @@ Fixpoint c_cmd (c: cmd) (l: nat) (fs: f_lookup) (vs: v_stack): (asm_appl * nat) 
     (asm1 +++ asm2, l2)
   | Alloc n e =>
     let/d '(asm1, l1) := c_exp e l vs in
-    let/d asm2_len := app_list_length (c_alloc vs) in
+    let/d asm2_len := appl_len (c_alloc vs) in
     let/d '(asm3, l3) := c_assign n (l1 + asm2_len) vs in
     (asm1 +++ c_alloc vs +++ asm3, l3)
   | GetChar n =>
@@ -438,21 +421,21 @@ Fixpoint c_cmd (c: cmd) (l: nat) (fs: f_lookup) (vs: v_stack): (asm_appl * nat) 
 Theorem c_cmd_equation: ltac2:(unfold_fix_type '@c_cmd).
 Proof. unfold_fix_proof '@c_cmd. Qed.
 
-Fixpoint all_binders (c: cmd): list name :=
+Fixpoint all_bdrs (c: cmd): list name :=
   match c with
   | Skip =>
     let/d l := [] in
     l
   | Seq c1 c2 => 
-    list_append (all_binders c1) (all_binders c2)
+    list_app (all_bdrs c1) (all_bdrs c2)
   | Assign n e => [n]
   | Update a e e' =>
     let/d l := [] in
     l
   | If t c1 c2 => 
-    list_append (all_binders c1) (all_binders c2)
+    list_app (all_bdrs c1) (all_bdrs c2)
   | While tst body => 
-    all_binders body
+    all_bdrs body
   | Call n f es => [n]
   | Return e =>
     let/d l := [] in
@@ -466,126 +449,126 @@ Fixpoint all_binders (c: cmd): list name :=
     let/d l := [] in
     l
   end.
-Theorem all_binders_equation: ltac2:(unfold_fix_type '@all_binders).
-Proof. unfold_fix_proof '@all_binders. Qed.
+Theorem all_bdrs_equation: ltac2:(unfold_fix_type '@all_bdrs).
+Proof. unfold_fix_proof '@all_bdrs. Qed.
 
-Fixpoint names_contain (l: list name) (a: name): bool :=
+Fixpoint names_in (l: list name) (a: name): bool :=
   match l with
   | nil => false
   | x :: l =>
     if (x =? a)%N then
       true
     else
-      names_contain l a
+      names_in l a
   end.
-Theorem names_contain_equation: ltac2:(unfold_fix_type '@names_contain).
-Proof. unfold_fix_proof '@names_contain. Qed.
+Theorem names_in_equation: ltac2:(unfold_fix_type '@names_in).
+Proof. unfold_fix_proof '@names_in. Qed.
 
-Fixpoint names_unique (l: list name) (acc: list name): list name :=
+Fixpoint nms_uniq (l: list name) (acc: list name): list name :=
   match l with
   | nil => acc
   | x :: xs =>
-    let/d acc_contains_x := names_contain acc x in
-    if acc_contains_x then
-      names_unique xs acc
+    let/d x_in_acc := names_in acc x in
+    if x_in_acc then
+      nms_uniq xs acc
     else
-      names_unique xs (x :: acc)
+      nms_uniq xs (x :: acc)
   end.
-Theorem names_unique_equation: ltac2:(unfold_fix_type '@names_unique).
-Proof. unfold_fix_proof '@names_unique. Qed.
+Theorem nms_uniq_equation: ltac2:(unfold_fix_type '@nms_uniq).
+Proof. unfold_fix_proof '@nms_uniq. Qed.
 
-Definition unique_binders (c: cmd): list name :=
-  names_unique (all_binders c) [].
+Definition bdrs_unq (c: cmd): list name :=
+  nms_uniq (all_bdrs c) [].
 
-Fixpoint make_vs_from_binders (binders: list name): v_stack :=
+Fixpoint bdrs_vs (binders: list name): v_stack :=
   match binders with
   | nil => nil
   | b :: binders => 
-    Some b :: make_vs_from_binders binders
+    Some b :: bdrs_vs binders
   end.
-Theorem make_vs_from_binders_equation: ltac2:(unfold_fix_type '@make_vs_from_binders).
-Proof. unfold_fix_proof '@make_vs_from_binders. Qed.
+Theorem bdrs_vs_equation: ltac2:(unfold_fix_type '@bdrs_vs).
+Proof. unfold_fix_proof '@bdrs_vs. Qed.
 
-Fixpoint filter_name (a: name) (l: list name): list name :=
+Fixpoint fltr_nms (a: name) (l: list name): list name :=
   match l with
   | nil => let/d l := [] in l
   | x :: xs =>
     if (a =? x)%N then
-      filter_name a xs
+      fltr_nms a xs
     else
-      x :: filter_name a xs
+      x :: fltr_nms a xs
   end.
-Theorem filter_name_equation: ltac2:(unfold_fix_type '@filter_name).
-Proof. unfold_fix_proof '@filter_name. Qed.
+Theorem fltr_nms_equation: ltac2:(unfold_fix_type '@fltr_nms).
+Proof. unfold_fix_proof '@fltr_nms. Qed.
 
-Fixpoint remove_names (l1 l2: list name): list name :=
+Fixpoint rm_nms (l1 l2: list name): list name :=
   match l1 with
   | nil => l2
   | x :: xs => 
-    remove_names xs (filter_name x l2)
+    rm_nms xs (fltr_nms x l2)
   end.
-Theorem remove_names_equation: ltac2:(unfold_fix_type '@remove_names).
-Proof. unfold_fix_proof '@remove_names. Qed.
+Theorem rm_nms_equation: ltac2:(unfold_fix_type '@rm_nms).
+Proof. unfold_fix_proof '@rm_nms. Qed.
 
-Definition get_vs_binders (vs_after_pushes: v_stack) (vs_binders: v_stack): v_stack :=
-  let/d cond := even_len vs_after_pushes in
+Definition vs_bdrs (vs_after: v_stack) (vs_bdrs: v_stack): v_stack :=
+  let/d cond := even_len vs_after in
   if cond then
-    let/d vs_binders1 := list_append vs_binders [None] in
-    vs_binders1
+    let/d vs_bind1 := list_app vs_bdrs [None] in
+    vs_bind1
   else
-    vs_binders.
+    vs_bdrs.
 
-Definition c_declare_binders (v_names: list name) (c: cmd): (asm_appl * v_stack) :=
-  let/d vs_binders := make_vs_from_binders (remove_names v_names (unique_binders c)) in
-  let/d vs_after_pushes := list_append (c_pushes_vs v_names) vs_binders in
-  let/d cond := even_len vs_after_pushes in
-  let/d vs_binders1 := get_vs_binders vs_after_pushes vs_binders in
-  (List [Sub_RSP (List.length vs_binders1)], vs_binders1).
+Definition c_bdrs (v_names: list name) (c: cmd): (asm_appl * v_stack) :=
+  let/d vs_bind := bdrs_vs (rm_nms v_names (bdrs_unq c)) in
+  let/d vs_after := list_app (push_vs v_names) vs_bind in
+  let/d cond := even_len vs_after in
+  let/d vs_bind1 := vs_bdrs vs_after vs_bind in
+  (List [Sub_RSP (List.length vs_bind1)], vs_bind1).
 
 (** Compiles a single function definition into assembly code. *)
 Definition c_fundef (fundef: func) (l: nat) (fs: f_lookup): (asm_appl * nat) :=
   match fundef with
   | Func n v_names body =>
-    let/d '(asm0, vs_binders1) := c_declare_binders v_names body in
-    let/d l0 := l + app_list_length asm0 in
+    let/d '(asm0, vs_bind1) := c_bdrs v_names body in
+    let/d l0 := l + appl_len asm0 in
     let/d '(asm1, vs1, l1) := c_pushes v_names l0 in
-    let/d '(asm2, l2) := c_cmd body l1 fs (list_append vs1 vs_binders1) in
+    let/d '(asm2, l2) := c_cmd body l1 fs (list_app vs1 vs_bind1) in
     (asm0 +++ asm1 +++ asm2, l2)
   end.
 
-Definition get_funcs (prg: prog): list func :=
+Definition get_funs (prg: prog): list func :=
   match prg with
   | Program funcs => funcs
   end.
 
-Definition name_of_func (f: func) : name :=
+Definition func_nm (f: func) : name :=
   match f with
   | Func n _ _ => n
   end.
 
 (* Compiles a list of function declarations into assembly instructions *)
-Fixpoint c_fundefs (ds: list func) (l: nat) (fs: f_lookup): (asm_appl * list (name * nat) * nat) :=
+Fixpoint c_fndefs (ds: list func) (l: nat) (fs: f_lookup): (asm_appl * list (name * nat) * nat) :=
   match ds with
   | [] => 
     (List [], fs, l)
   | d :: ds' =>
-    let/d fname := name_of_func d in
+    let/d fname := func_nm d in
     let/d '(c1, l1) := c_fundef d (l + 1) fs in
-    let/d '(c2, fs', l2) := c_fundefs ds' (l1 + 1) fs in
-    let/d comment := List [Comment (N2ascii_default fname)] in
+    let/d '(c2, fs', l2) := c_fndefs ds' (l1 + 1) fs in
+    let/d comment := List [Comment (N2asciid fname)] in
     (comment +++ c1 +++ List [Ret] +++ c2, (fname, (l + 1)) :: fs', l2)
   end.
-Theorem c_fundefs_equation: ltac2:(unfold_fix_type '@c_fundefs).
-Proof. unfold_fix_proof '@c_fundefs. Qed.
+Theorem c_fndefs_equation: ltac2:(unfold_fix_type '@c_fndefs).
+Proof. unfold_fix_proof '@c_fndefs. Qed.
 
 (* Generates the complete assembly code for a given program *)
 Definition codegen (prog : prog) : asm :=
-  let/d funs := get_funcs prog in
-  let/d init_list := List (init 0) in
-  let/d init_l := app_list_length init_list in
-  let/d '(_, fs, _) := c_fundefs funs init_l [] in
-  let/d '(asm1, _, _) := c_fundefs funs init_l fs in
+  let/d funs := get_funs prog in
+  let/d init_lst := List (init 0) in
+  let/d init_len := appl_len init_lst in
+  let/d '(_, fs, _) := c_fndefs funs init_len [] in
+  let/d '(asm1, _, _) := c_fndefs funs init_len fs in
   (*                        vvv (name_of_string ("main"%string)) *)
   let/d main_l := lookup fs 1835100526%N in
-  let/d main_init_list := List (init main_l) in
-  flatten (main_init_list +++ asm1).
+  let/d asm0 := List (init main_l) in
+  flatten (asm0 +++ asm1).
