coq/theories/parsing/Parser.v
@@ -18,120 +18,103 @@ Open Scope string.
 
 (* lexing *)
 
-Fixpoint read_num (l_h: (ascii * ascii)) (f_x: (N * N)) (acc: N) (cs: list ascii): (N * list ascii) :=
-  let/d '(l, h) := l_h in
-  let/d '(f, x) := f_x in
+Fixpoint read_num (l h: ascii) (f x: N) (acc: N) (cs: list ascii): (N * list ascii) :=
   match cs return (N * list ascii) with
   [] => 
-    let/d empty_list := [] in
-    let/d result := (acc, empty_list) in
+    let/d empty := [] in
+    let/d result := (acc, empty) in
     result
   | c :: cs1 =>
-    let/d l_ascii := N_of_ascii l in
-    let/d c_ascii := N_of_ascii c in
-    let/d h_ascii := N_of_ascii h in
-    if (c_ascii <? l_ascii)%N then
+    let/d l_asc := N_of_ascii l in
+    let/d c_asc := N_of_ascii c in
+    let/d h_asc := N_of_ascii h in
+    if (c_asc <? l_asc)%N then
       let/d result := (acc, cs) in
       result
     else
-      if (h_ascii <? c_ascii)%N then
+      if (h_asc <? c_asc)%N then
         let/d result := (acc, cs) in
         result
       else
-        let/d f_mult_acc := acc * f in
-        let/d c_minus_x := c_ascii - x in
-        let/d new_acc := f_mult_acc + c_minus_x in
-        let/d result := read_num l_h f_x new_acc cs1 in
+        let/d f_mult := acc * f in
+        let/d c_min_x := c_asc - x in
+        let/d new_acc := f_mult + c_min_x in
+        let/d result := read_num l h f x new_acc cs1 in
         result
   end.
 
 (* read_num ("0"%char, "9"%char) (10, N_of_ascii "0"%char) *)
-Fixpoint read_num_numeric (acc: N) (cs: list ascii): (N * list ascii) :=
-  match cs return (N * list ascii) with
+Fixpoint read_nmc (acc: N) (cs: list ascii) (len: N): (N * list ascii * N) :=
+  match cs return (N * list ascii * N) with
   [] => 
-    let/d empty_list := [] in
-    let/d result := (acc, empty_list) in
-    result
+    let/d empty := [] in
+    (acc, empty, len)
   | c :: cs1 =>
-    let/d l_ascii := N_of_ascii "0"%char in
-    let/d c_ascii := N_of_ascii c in
-    let/d h_ascii := N_of_ascii "9"%char in
-    if (c_ascii <? l_ascii)%N then
-      let/d result := (acc, cs) in
-      result
+    let/d l_asc := N_of_ascii "0"%char in
+    let/d c_asc := N_of_ascii c in
+    let/d h_asc := N_of_ascii "9"%char in
+    if (c_asc <? l_asc)%N then
+      (acc, cs, len)
     else
-      if (h_ascii <? c_ascii)%N then
-        let/d result := (acc, cs) in
-        result
+      if (h_asc <? c_asc)%N then
+        (acc, cs, len)
       else
-        let/d f_mult_acc := acc * 10 in
-        let/d c_minus_x := c_ascii - (N_of_ascii "0"%char) in
-        let/d new_acc := f_mult_acc + c_minus_x in
-        let/d result := read_num_numeric new_acc cs1 in
-        result
+        let/d f_mult := acc * 10 in
+        let/d c_min_x := c_asc - (N_of_ascii "0"%char) in
+        let/d new_acc := f_mult + c_min_x in
+        read_nmc new_acc cs1 (len + 1)
   end.
-Theorem read_num_numeric_equation: ltac2:(unfold_fix_type '@read_num_numeric).
-Proof. unfold_fix_proof '@read_num_numeric. Qed.
+Theorem read_nmc_equation: ltac2:(unfold_fix_type '@read_nmc).
+Proof. unfold_fix_proof '@read_nmc. Qed.
 
 (* read_num ("*"%char, "z"%char) (256, 0) *)
-Fixpoint read_num_alpha (acc: N) (cs: list ascii): (N * list ascii) :=
-  match cs return (N * list ascii) with
+Fixpoint read_alp (acc: N) (cs: list ascii) (len: N): (N * list ascii * N) :=
+  match cs return (N * list ascii * N) with
   [] => 
-    let/d empty_list := [] in
-    let/d result := (acc, empty_list) in
-    result
+    let/d empl := [] in
+    (acc, empl, len)
   | c :: cs1 =>
-    let/d l_ascii := N_of_ascii "*"%char in
-    let/d c_ascii := N_of_ascii c in
-    let/d h_ascii := N_of_ascii "z"%char in
-    if (c_ascii <? l_ascii)%N then
-      let/d result := (acc, cs) in
-      result
+    let/d l_asc := N_of_ascii "*"%char in
+    let/d c_asc := N_of_ascii c in
+    let/d h_asc := N_of_ascii "z"%char in
+    if (c_asc <? l_asc)%N then
+      (acc, cs, len)
     else
-      if (h_ascii <? c_ascii)%N then
-        let/d result := (acc, cs) in
-        result
+      if (h_asc <? c_asc)%N then
+        (acc, cs, len)
       else
-        let/d f_mult_acc := acc * 256 in
-        let/d c_minus_x := c_ascii in
-        let/d new_acc := f_mult_acc + c_minus_x in
-        let/d result := read_num_alpha new_acc cs1 in
-        result
+        let/d f_mult := acc * 256 in
+        let/d new_acc := f_mult + c_asc in
+        read_alp new_acc cs1 (len + 1)
   end.
-Theorem read_num_alpha_equation: ltac2:(unfold_fix_type '@read_num_alpha).
-Proof. unfold_fix_proof '@read_num_alpha. Qed.
+Theorem read_alp_equation: ltac2:(unfold_fix_type '@read_alp).
+Proof. unfold_fix_proof '@read_alp. Qed.
 
-Fixpoint end_line (cs: list ascii) :=
+Fixpoint end_line (cs: list ascii) (len: N): (list ascii * N) :=
   match cs with
   | [] => 
-    let/d empty_list := [] in
-    empty_list
+    ([], len)
   | c :: cs =>
-    let/d newline_char := "010"%char in
-    if Ascii.eqb c newline_char then 
-      cs 
-    else 
-      let/d result := end_line cs in
-      result
+    let/d newline := "010"%char in
+    if Ascii.eqb c newline then 
+      (cs, len + 1)
+    else
+      end_line cs (len + 1)
   end.
 Theorem end_line_equation: ltac2:(unfold_fix_type '@end_line).
 Proof. unfold_fix_proof '@end_line. Qed.
 
-Definition q_from_nat (n: nat) (arg: N) :=
+Definition q_of_nat (n: nat) (arg: N) :=
   match n with
   | 0%nat =>
-    let/d res := NUM arg in
-    res
+    NUM arg
   | _ =>
-    let/d res := QUOTE arg in
-    res
+    QUOTE arg
   end.
 
-Fixpoint lex (q: nat) (cs: list ascii) (acc: list token) (fuel: nat): option (list token) :=
+Fixpoint lex (q: nat) (cs: list ascii) (cs_len: N) (acc: list token) (fuel: nat): option (list token) :=
   match cs with
-  | [] => 
-    let/d result := Some acc in
-    result
+  | [] => Some acc
   | c :: cs =>
     match fuel with
     | 0%nat => 
@@ -139,63 +122,45 @@ Fixpoint lex (q: nat) (cs: list ascii) (acc: list token) (fuel: nat): option (li
       result
     | S fuel =>
       if Ascii.eqb c " "%char then
-        let/d result := lex 0 cs acc fuel in
-        result
+        lex 0 cs (cs_len - 1) acc fuel
       else if Ascii.eqb c "009"%char then
-        let/d result := lex 0 cs acc fuel in
-        result
+        lex 0 cs (cs_len - 1) acc fuel
       else if Ascii.eqb c "010"%char then
-        let/d result := lex 0 cs acc fuel in
-        result
+        lex 0 cs (cs_len - 1) acc fuel
       else if Ascii.eqb c "#"%char then 
-        let/d line_end := end_line cs in
-        let/d result := lex 0 line_end acc fuel in
-        result
+        let/d '(cs1, len) := end_line cs 0 in
+        lex 0 cs1 (cs_len - len) acc fuel
       else if Ascii.eqb c "."%char then 
-        let/d dot_token := DOT in
-        let/d new_acc := dot_token :: acc in
-        let/d result := lex 0 cs new_acc fuel in
-        result
+        let/d new_acc := DOT :: acc in
+        lex 0 cs (cs_len - 1) new_acc fuel
       else if Ascii.eqb c "("%char then 
-        let/d open_token := OPEN in
-        let/d new_acc := open_token :: acc in
-        let/d result := lex 0 cs new_acc fuel in
-        result
+        let/d new_acc := OPEN :: acc in
+        lex 0 cs (cs_len - 1) new_acc fuel
       else if Ascii.eqb c ")"%char then 
-        let/d close_token := CLOSE in
-        let/d new_acc := close_token :: acc in
-        let/d result := lex 0 cs new_acc fuel in
-        result
+        let/d new_acc := CLOSE :: acc in
+        lex 0 cs (cs_len - 1) new_acc fuel
       else if Ascii.eqb c "'"%char then 
-        let/d result := lex 1 cs acc fuel in
-        result
+        lex 1 cs (cs_len - 1) acc fuel
       else
-        let/d c_cons_cs := c :: cs in
-        let/d digit_result := read_num_numeric 0 c_cons_cs in
-        match digit_result return (option (list token)) with
-        | (n, rest) =>
-          let/d rest_length := list_length rest in
-          let/d original_length := list_length c_cons_cs in
-          if Nat.eqb rest_length original_length then
-            let/d alpha_result := read_num_alpha 0 c_cons_cs in
-            match alpha_result return (option (list token)) with
-            | (n2, rest2) =>
-              let/d rest2_length := list_length rest2 in
-              let/d original_length2 := list_length c_cons_cs in
-              if Nat.eqb rest2_length original_length2 then
-                let/d result := lex 0 cs acc fuel in
-                result
+        let/d c_cons := c :: cs in
+        let/d digitr := read_nmc 0 c_cons 0 in
+        match digitr return (option (list token)) with
+        | (n, rest, len) =>
+          if N.eqb len 0 then
+            let/d alphar := read_alp 0 c_cons 0 in
+            match alphar return (option (list token)) with
+            | (n2, rest2, len2) =>
+              if N.eqb len2 0 then
+                lex 0 cs (cs_len - 1) acc fuel
               else
-                let/d q_token2 := q_from_nat q n2 in
-                let/d new_acc2 := q_token2 :: acc in
-                let/d result := lex 0 rest2 new_acc2 fuel in
-                result
+                let/d q_tok2 := q_of_nat q n2 in
+                let/d new_acc2 := q_tok2 :: acc in
+                lex 0 rest2 (cs_len - len2) new_acc2 fuel
             end
           else
-            let/d q_token := q_from_nat q n in
-            let/d new_acc := q_token :: acc in
-            let/d result := lex 0 rest new_acc fuel in
-            result
+            let/d q_tok := q_of_nat q n in
+            let/d new_acc := q_tok :: acc in
+            lex 0 rest (cs_len - len) new_acc fuel
         end
     end
   end.
@@ -203,9 +168,9 @@ Theorem lex_equation: ltac2:(unfold_fix_type '@lex).
 Proof. unfold_fix_proof '@lex. Qed.
 
 Definition lexer_i (input: list ascii): option (list token) :=
-  let/d len := list_length input in
-  let/d empty_list := [] in
-  lex 0 input empty_list len.
+  let/d len := list_len input in
+  let/d empty := [] in
+  lex 0 input (N.of_nat len) empty len.
 
 Definition lexer (input: list ascii): list token :=
   let/d r := lexer_i input in
@@ -219,45 +184,34 @@ Definition lexer (input: list ascii): list token :=
 (* parsing *)
 
 Definition quote (n: N) :=
-  let/d quote_enc := name_enc "'" in
-  let/d quote_num := Num quote_enc in
-  let/d n_num := Num n in
-  let/d pair_list := [quote_num; n_num] in
-  let/d result := FunValues.vlist pair_list in
-  result.
+  FunValues.vlist [Num (name_enc "'"); Num n].
 
-Fixpoint parse (ts: list token) (x: Value) (stck: list Value) :=
+Fixpoint parse (ts: list token) (x: Value) (stck: list Value): Value :=
   match ts with
   | [] => x
   | (CLOSE :: rest) => 
-    let/d zero_num := Num 0 in
+    let/d zero := Num 0 in
     let/d x_cons_s := x :: stck in
-    let/d result := parse rest zero_num x_cons_s in
-    result
+    parse rest zero x_cons_s
   | (OPEN :: rest) =>
     match stck with
     | [] => 
-      let/d result := parse rest x stck in
-      result
+      parse rest x stck
     | (y :: ys) => 
-      let/d pair_x_y := Pair x y in
-      let/d result := parse rest pair_x_y ys in
-      result
+      let/d pair_xy := Pair x y in
+      parse rest pair_xy ys
     end
   | (NUM n :: rest) => 
     let/d n_num := Num n in
-    let/d pair_n_x := Pair n_num x in
-    let/d result := parse rest pair_n_x stck in
-    result
+    let/d pair_nx := Pair n_num x in
+    parse rest pair_nx stck
   | (QUOTE n :: rest) => 
-    let/d quote_n := quote n in
-    let/d pair_quote_x := Pair quote_n x in
-    let/d result := parse rest pair_quote_x stck in
-    result
+    let/d q_n := quote n in
+    let/d pair_qx := Pair q_n x in
+    parse rest pair_qx stck
   | (DOT :: rest) => 
-    let/d vhead_x := FunValues.vhead x in
-    let/d result := parse rest vhead_x stck in
-    result
+    let/d vhead := FunValues.vhead x in
+    parse rest vhead stck
   end.
 Theorem parse_equation: ltac2:(unfold_fix_type '@parse).
 Proof. unfold_fix_proof '@parse. Qed.
@@ -267,86 +221,69 @@ Proof. unfold_fix_proof '@parse. Qed.
 Fixpoint v2list (v: FunValues.Value) :=
   match v with
   | Num _ => 
-    let/d empty_list := [] in
-    empty_list
+    let/d empty := [] in
+    empty
   | Pair v1 v2 =>
-    let/d v2_list := v2list v2 in
-    let/d result := v1 :: v2_list in
-    result
+    let/d v2_lst := v2list v2 in
+    v1 :: v2_lst
   end.
 Theorem v2list_equation: ltac2:(unfold_fix_type '@v2list).
 Proof. unfold_fix_proof '@v2list. Qed.
 
 Definition num2exp (n: N): exp :=
-  let/d is_upper := vis_upper n in
-  if is_upper then
+  let/d is_up := vupper n in
+  if is_up then
     (*  vvvvvvvvvvvvvvvvvvvv (2 ^ 64 - 1) *)
     if (18446744073709551615 <? n)%N then
-      let/d result := Const  (word.of_Z (Z.of_N 0)) in (* fail? *)
-      result
+      ImpSyntax.Const (word.of_Z (Z.of_N 0)) (* fail? *)
     else
-      (let/d word_val := word.of_Z (Z.of_N n) in
-      let/d result := ImpSyntax.Const word_val in
-      result)
+      ImpSyntax.Const (word.of_Z (Z.of_N n))
   else 
-    let/d result := Var n in
-    result.
+    Var n.
 
 Fixpoint v2exp (v: Value): ImpSyntax.exp :=
   match v with
   | Num n => 
-    let/d result := num2exp n in
-    result
+    num2exp n
   | Pair v0 v1 =>
     let/d n := vgetNum v0 in (* this can fail? *)
     match v1 return ImpSyntax.exp with
     | Num _ => 
-      let/d result := num2exp n in (* fail? *)
-      result
+      num2exp n (* fail? *)
     | Pair v1 v2 =>
       if N.eqb n (name_enc "'") then 
-        let/d v1_num := vgetNum v1 in
+        let/d v1_n := vgetNum v1 in
         (*  vvvvvvvvvvvvvvvvvvvv (2 ^ 64 - 1) *)
-        if (18446744073709551615 <? v1_num)%N then
-          let/d result := Const  (word.of_Z (Z.of_N 0)) in (* fail? *)
-          result
+        if (18446744073709551615 <? v1_n)%N then
+          ImpSyntax.Const (word.of_Z (Z.of_N 0)) (* fail? *)
         else
-          (let/d word_val := word.of_Z (Z.of_N v1_num) in
-          let/d result := ImpSyntax.Const word_val in
-          result)
+          ImpSyntax.Const (word.of_Z (Z.of_N v1_n))
       else if N.eqb n (name_enc "var") then 
-        let/d v1_num := vgetNum v1 in
-        let/d result := Var v1_num in
-        result
+        let/d v1_n := vgetNum v1 in
+        Var v1_n
       else
         match v2 with
         | Num _ => 
-          let/d result := num2exp n in (* fail? *)
-          result
+          num2exp n (* fail? *)
         | Pair v2 v3 =>
           if N.eqb n (name_enc "+") then 
-            let/d v1_exp := v2exp v1 in
-            let/d v2_exp := v2exp v2 in
-            let/d result := Add v1_exp v2_exp in
-            result
+            let/d v1_e := v2exp v1 in
+            let/d v2_e := v2exp v2 in
+            Add v1_e v2_e
           else if N.eqb n (name_enc "-") then 
-            let/d v1_exp := v2exp v1 in
-            let/d v2_exp := v2exp v2 in
-            let/d result := Sub v1_exp v2_exp in
-            result
+            let/d v1_e := v2exp v1 in
+            let/d v2_e := v2exp v2 in
+            Sub v1_e v2_e
           else if N.eqb n (name_enc "div") then 
-            let/d v1_exp := v2exp v1 in
-            let/d v2_exp := v2exp v2 in
-            let/d result := Div v1_exp v2_exp in
-            result
+            let/d v1_e := v2exp v1 in
+            let/d v2_e := v2exp v2 in
+            Div v1_e v2_e
           else if N.eqb n (name_enc "read") then 
-            let/d v1_exp := v2exp v1 in
-            let/d v2_exp := v2exp v2 in
-            let/d result := Read v1_exp v2_exp in
-            result
+            let/d v1_e := v2exp v1 in
+            let/d v2_e := v2exp v2 in
+            Read v1_e v2_e
           else
-            let/d result := num2exp n in (* fail? *)
-            result
+            num2exp n (* fail? *)
         end
     end
   end.
@@ -356,76 +293,65 @@ Proof. unfold_fix_proof '@v2exp. Qed.
 Fixpoint vs2exps (v: list Value): list ImpSyntax.exp :=
   match v with
   | [] => 
-    let/d empty_list := [] in
-    empty_list
+    let/d empl := [] in
+    empl
   | v1 :: vs =>
-    let/d v1_exp := v2exp v1 in
-    let/d vs_exps := vs2exps vs in
-    let/d result := v1_exp :: vs_exps in
-    result
+    let/d v1_e := v2exp v1 in
+    let/d vs_e := vs2exps vs in
+    v1_e :: vs_e
   end.
 Theorem vs2exps_equation: ltac2:(unfold_fix_type '@vs2exps).
 Proof. unfold_fix_proof '@vs2exps. Qed.
 
 Definition v2cmp (v: Value): ImpSyntax.cmp :=
-  let/d v_num := vgetNum v in
-  if N.eqb v_num (name_enc "<") then 
-    let/d res := Less in
-    res 
-  else if N.eqb v_num (name_enc "=") then 
-    let/d res := Equal in
-    res
+  let/d v_n := vgetNum v in
+  if N.eqb v_n (name_enc "<") then 
+    Less
+  else if N.eqb v_n (name_enc "=") then 
+    Equal
   else
-    let/d res := Less in
-    res. (* fail? *)
+    Less. (* fail? *)
 
 Fixpoint v2test (v: Value): ImpSyntax.test :=
   match v with
   | Num _ => 
-    let/d zero_word := word.of_Z (Z.of_N 0) in
-    let/d zero_const := Const zero_word in
+    let/d zero_w := word.of_Z (Z.of_N 0) in
+    let/d zero_c := Const zero_w in
     let/d less := Less in
-    let/d result := Test less zero_const zero_const in (* fail? *)
-    result
+    Test less zero_c zero_c (* fail? *)
   | Pair v0 v1 =>
     let/d n := vgetNum v0 in (* this can fail? *)
     match v1 return ImpSyntax.test with
     | Num _ => 
-      let/d zero_word := word.of_Z (Z.of_N 0) in
-      let/d zero_const := Const zero_word in
+      let/d zero_w := word.of_Z (Z.of_N 0) in
+      let/d zero_c := Const zero_w in
       let/d less := Less in
-      let/d result := Test less zero_const zero_const in (* fail? *)
-      result
+      Test less zero_c zero_c (* fail? *)
     | Pair v1 v2 =>
       if N.eqb n (name_enc "not") then 
-        let/d v1_test := v2test v1 in
-        let/d result := Not v1_test in
-        result
+        let/d v1_t := v2test v1 in
+        Not v1_t
       else
         match v2 with
         | Num _ => 
-          let/d zero_word := word.of_Z (Z.of_N 0) in
-          let/d zero_const := Const zero_word in
+          let/d zero_w := word.of_Z (Z.of_N 0) in
+          let/d zero_c := Const zero_w in
           let/d less := Less in
-          let/d result := Test less zero_const zero_const in (* fail? *)
-          result
+          Test less zero_c zero_c (* fail? *)
         | Pair v2 v3 =>
           if N.eqb n (name_enc "and") then 
-            let/d v1_test := v2test v1 in
-            let/d v2_test := v2test v2 in
-            let/d result := And v1_test v2_test in
-            result
+            let/d v1_t := v2test v1 in
+            let/d v2_t := v2test v2 in
+            And v1_t v2_t
           else if N.eqb n (name_enc "or") then 
-            let/d v1_test := v2test v1 in
-            let/d v2_test := v2test v2 in
-            let/d result := Or v1_test v2_test in
-            result
+            let/d v1_t := v2test v1 in
+            let/d v2_t := v2test v2 in
+            Or v1_t v2_t
           else
-            let/d v0_cmp := v2cmp v0 in
-            let/d v1_exp := v2exp v1 in
-            let/d v2_exp := v2exp v2 in
-            let/d result := Test v0_cmp v1_exp v2_exp in
-            result
+            let/d v0_c := v2cmp v0 in
+            let/d v1_e := v2exp v1 in
+            let/d v2_e := v2exp v2 in
+            Test v0_c v1_e v2_e
         end
     end
   end.
@@ -442,13 +368,11 @@ Fixpoint v2cmd (v: Value): ImpSyntax.cmd :=
     if iPv0 then
       let/d iNv1 := visNum v1 in
       if iNv1 then
-        let/d result := v2cmd v0 in
-        result
+        v2cmd v0
       else
-        let/d v0_cmd := v2cmd v0 in
-        let/d v1_cmd := v2cmd v1 in
-        let/d result := Seq v0_cmd v1_cmd in
-        result
+        let/d v0_c := v2cmd v0 in
+        let/d v1_c := v2cmd v1 in
+        Seq v0_c v1_c
     else
       let/d n := vgetNum v0 in
       if N.eqb n (name_enc "abort") then
@@ -461,17 +385,14 @@ Fixpoint v2cmd (v: Value): ImpSyntax.cmd :=
           res
         | Pair v1 v2 =>
           if N.eqb n (name_enc "return") then
-            let/d v1_exp := v2exp v1 in
-            let/d result := Return v1_exp in
-            result
+            let/d v1_e := v2exp v1 in
+            Return v1_e
           else if N.eqb n (name_enc "getchar") then
-            let/d v1_num := vgetNum v1 in
-            let/d result := GetChar v1_num in
-            result
+            let/d v1_n := vgetNum v1 in
+            GetChar v1_n
           else if N.eqb n (name_enc "putchar") then
-            let/d v1_exp := v2exp v1 in
-            let/d result := PutChar v1_exp in
-            result
+            let/d v1_e := v2exp v1 in
+            PutChar v1_e
           else
             match v2 with
             | Num _ => (* fail? *)
@@ -479,57 +400,49 @@ Fixpoint v2cmd (v: Value): ImpSyntax.cmd :=
               res
             | Pair v2 v3 =>
               if N.eqb n (name_enc "assign") then
-                let/d v1_num := vgetNum v1 in
-                let/d v2_exp := v2exp v2 in
-                let/d result := Assign v1_num v2_exp in
-                result
+                let/d v1_n := vgetNum v1 in
+                let/d v2_e := v2exp v2 in
+                Assign v1_n v2_e
               else if N.eqb n (name_enc "while") then
-                let/d v1_test := v2test v1 in
-                let/d v2_cmd := v2cmd v2 in
-                let/d result := While v1_test v2_cmd in
-                result
+                let/d v1_t := v2test v1 in
+                let/d v2_c := v2cmd v2 in
+                While v1_t v2_c
               else if N.eqb n (name_enc "alloc") then
-                let/d v1_num := vgetNum v1 in
-                let/d v2_exp := v2exp v2 in
-                let/d result := Alloc v1_num v2_exp in
-                result
+                let/d v1_n := vgetNum v1 in
+                let/d v2_e := v2exp v2 in
+                Alloc v1_n v2_e
               else
                 match v3 with
                 | Num _ =>
-                  let/d v0_num := vgetNum v0 in
-                  let/d v1_num := vgetNum v1 in
-                  let/d v2_list := v2list v2 in
-                  let/d v2_exps := vs2exps v2_list in
-                  let/d result := Call v0_num v1_num v2_exps in
-                  result
+                  let/d v0_n := vgetNum v0 in
+                  let/d v1_n := vgetNum v1 in
+                  let/d v2_lst := v2list v2 in
+                  let/d v2_e := vs2exps v2_lst in
+                  Call v0_n v1_n v2_e
                 | Pair v3 v4 =>
                   if N.eqb n (name_enc "update") then
-                    let/d v1_exp := v2exp v1 in
-                    let/d v2_exp := v2exp v2 in
-                    let/d v3_exp := v2exp v3 in
-                    let/d result := Update v1_exp v2_exp v3_exp in
-                    result
+                    let/d v1_e := v2exp v1 in
+                    let/d v2_e := v2exp v2 in
+                    let/d v3_e := v2exp v3 in
+                    Update v1_e v2_e v3_e
                   else if N.eqb n (name_enc "if") then
-                    let/d v1_test := v2test v1 in
-                    let/d v2_cmd := v2cmd v2 in
-                    let/d v3_cmd := v2cmd v3 in
-                    let/d result := If v1_test v2_cmd v3_cmd in
-                    result
+                    let/d v1_t := v2test v1 in
+                    let/d v2_c := v2cmd v2 in
+                    let/d v3_c := v2cmd v3 in
+                    If v1_t v2_c v3_c
                   else if N.eqb n (name_enc "call") then
-                    let/d v1_num := vgetNum v1 in
-                    let/d v2_num := vgetNum v2 in
-                    let/d v3_list := v2list v3 in
-                    let/d v3_exps := vs2exps v3_list in
-                    let/d result := Call v1_num v2_num v3_exps in
-                    result
+                    let/d v1_n := vgetNum v1 in
+                    let/d v2_n := vgetNum v2 in
+                    let/d v3_lst := v2list v3 in
+                    let/d v3_e := vs2exps v3_lst in
+                    Call v1_n v2_n v3_e
                   else
-                    let/d v0_num := vgetNum v0 in
-                    let/d v1_num := vgetNum v1 in
-                    let/d v2_v3_pair := Pair v2 v3 in
-                    let/d pair_list := v2list v2_v3_pair in
-                    let/d pair_exps := vs2exps pair_list in
-                    let/d result := Call v0_num v1_num pair_exps in
-                    result
+                    let/d v0_n := vgetNum v0 in
+                    let/d v1_n := vgetNum v1 in
+                    let/d v2_v3 := Pair v2 v3 in
+                    let/d pair_lst := v2list v2_v3 in
+                    let/d pair_e := vs2exps pair_lst in
+                    Call v0_n v1_n pair_e
                 end
             end
         end
@@ -540,59 +453,54 @@ Proof. unfold_fix_proof '@v2cmd. Qed.
 Fixpoint vs2args (vs: list Value) :=
   match vs with
   | [] => 
-    let/d empty_list := [] in
-    empty_list
+    let/d empl := [] in
+    empl
   | v :: vs =>
-    let/d v_num := vgetNum v in
-    let/d vs_args := vs2args vs in
-    let/d result := v_num :: vs_args in
+    let/d v_n := vgetNum v in
+    let/d vs_a := vs2args vs in
+    let/d result := v_n :: vs_a in
     result
   end.
 Theorem vs2args_equation: ltac2:(unfold_fix_type '@vs2args).
 Proof. unfold_fix_proof '@vs2args. Qed.
 
 Definition v2func (v: Value) :=
-  let/d vel1_v := vel1 v in
-  let/d func_name := vgetNum vel1_v in
-  let/d vel2_v := vel2 v in
-  let/d vel2_list := v2list vel2_v in
-  let/d args := vs2args vel2_list in
-  let/d vel3_v := vel3 v in
-  let/d body := v2cmd vel3_v in
-  let/d result := ImpSyntax.Func func_name args body in
-  result.
+  let/d vel1 := vel1 v in
+  let/d fname := vgetNum vel1 in
+  let/d vel2 := vel2 v in
+  let/d vel2_l := v2list vel2 in
+  let/d args := vs2args vel2_l in
+  let/d vel3 := vel3 v in
+  let/d body := v2cmd vel3 in
+  ImpSyntax.Func fname args body.
 
 Fixpoint v2funcs (vs: list Value) :=
   match vs with
   | [] => 
-    let/d empty_list := [] in
-    empty_list
+    let/d empl := [] in
+    empl
   | v :: vs =>
-    let/d v_func := v2func v in
-    let/d vs_funcs := v2funcs vs in
-    let/d result := v_func :: vs_funcs in
-    result
+    let/d v_f := v2func v in
+    let/d vs_f := v2funcs vs in
+    v_f :: vs_f
   end.
 Theorem v2funcs_equation: ltac2:(unfold_fix_type '@v2funcs).
 Proof. unfold_fix_proof '@v2funcs. Qed.
 
 Definition vs2prog (vs: list Value) :=
   let/d ds := v2funcs vs in
-  let/d result := ImpSyntax.Program ds in
-  result.
+  ImpSyntax.Program ds.
 
 (* entire parser *)
 
 Definition parser (tokens: list token): prog :=
-  let/d zero_num := Num 0 in
-  let/d empty_stack := [] in
-  let/d parsed_val := parse tokens zero_num empty_stack in
-  let/d val_list := v2list parsed_val in
-  let/d result := vs2prog val_list in
-  result.
+  let/d zero := Num 0 in
+  let/d empty_s := [] in
+  let/d parsed := parse tokens zero empty_s in
+  let/d val_lst := v2list parsed in
+  vs2prog val_lst.
 
 Definition str2imp (str: list ascii): ImpSyntax.prog :=
   let/d toks := lexer str in
   let/d prog := parser toks in
-  let/d result := prog in
-  result.
+  prog.
