coq/theories/derivations/CompilerUtilsDerivations.v
@@ -20,58 +20,58 @@ From Stdlib Require Import derive.Derive.
 From Stdlib Require Import Lia.
 From Ltac2 Require Import Ltac2.
 
-Derive nat_modulo_10_prog
-  in ltac2:(relcompile_tpe 'nat_modulo_10_prog 'nat_modulo_10 ['mul_nat_10])
-  as nat_modulo_10_prog_proof.
+Derive natmod10_prog
+  in ltac2:(relcompile_tpe 'natmod10_prog 'natmod10 ['mulnat10])
+  as natmod10_prog_proof.
 Proof.
   time relcompile.
   ltac1:(lia).
 Qed.
-Time Compute to_funs [nat_modulo_10_prog].
+Time Compute to_funs [natmod10_prog].
 
-Derive N_modulo_10_prog
-  in ltac2:(relcompile_tpe 'N_modulo_10_prog 'N_modulo_10 ['mul_N_10])
-  as N_modulo_10_prog_proof.
+Derive Nmod_10_prog
+  in ltac2:(relcompile_tpe 'Nmod_10_prog 'Nmod_10 ['mulN_10])
+  as Nmod_10_prog_proof.
 Proof.
   time relcompile.
   ltac1:(lia).
 Qed.
-Time Compute to_funs [N_modulo_10_prog].
+Time Compute to_funs [Nmod_10_prog].
 
-Derive N_modulo_256_prog
-  in ltac2:(relcompile_tpe 'N_modulo_256_prog 'N_modulo_256 ['mul_N_256])
-  as N_modulo_256_prog_proof.
+Derive Nmod_256_prog
+  in ltac2:(relcompile_tpe 'Nmod_256_prog 'Nmod_256 ['mulN_256])
+  as Nmod_256_prog_proof.
 Proof.
   time relcompile.
   ltac1:(lia).
 Qed.
-Time Compute to_funs [N_modulo_256_prog].
+Time Compute to_funs [Nmod_256_prog].
 
-Theorem string_append_equation: ltac2:(unfold_fix_type '@string_append).
-Proof. unfold_fix_proof '@string_append. Qed.
-Derive string_append_prog
-  in ltac2:(relcompile_tpe 'string_append_prog 'string_append [])
-  as string_append_prog_proof.
+Theorem str_app_equation: ltac2:(unfold_fix_type '@str_app).
+Proof. unfold_fix_proof '@str_app. Qed.
+Derive str_app_prog
+  in ltac2:(relcompile_tpe 'str_app_prog 'str_app [])
+  as str_app_prog_proof.
 Proof.
   time relcompile.
 Qed.
-Time Compute to_funs [string_append_prog].
+Time Compute to_funs [str_app_prog].
 
-Theorem num2str_f_equation: ltac2:(unfold_fix_type '@num2str_f).
-Proof. unfold_fix_proof '@num2str_f. Qed.
+Theorem num2strf_equation: ltac2:(unfold_fix_type '@num2strf).
+Proof. unfold_fix_proof '@num2strf. Qed.
 
-Derive num2str_f_prog
-  in ltac2:(relcompile_tpe 'num2str_f_prog 'num2str_f ['nat_modulo_10])
-  as num2str_f_prog_proof.
+Derive num2strf_prog
+  in ltac2:(relcompile_tpe 'num2strf_prog 'num2strf ['natmod10])
+  as num2strf_prog_proof.
 Proof.
   time relcompile.
   all: ltac1:(try lia).
-  all: subst; rewrite nat_modulo_10_spec in *; specialize nat_modulo_le with (n := n) (m := 10); ltac1:(lia).
+  all: subst; rewrite natmod10_spec in *; specialize nat_mod_le with (n := n) (m := 10); ltac1:(lia).
 Qed.
-Time Compute to_funs [num2str_f_prog].
+Time Compute to_funs [num2strf_prog].
 
 Derive num2str_prog
-  in ltac2:(relcompile_tpe 'num2str_prog 'num2str ['num2str_f])
+  in ltac2:(relcompile_tpe 'num2str_prog 'num2str ['num2strf])
   as num2str_prog_proof.
 Proof.
   time relcompile.
@@ -82,13 +82,13 @@ Theorem N2str_f_equation: ltac2:(unfold_fix_type '@N2str_f).
 Proof. unfold_fix_proof '@N2str_f. Qed.
 
 Derive N2str_f_prog
-  in ltac2:(relcompile_tpe 'N2str_f_prog 'N2str_f ['N_modulo_10])
+  in ltac2:(relcompile_tpe 'N2str_f_prog 'N2str_f ['Nmod_10])
   as N2str_f_prog_proof.
 Proof.
   time relcompile.
   all: ltac1:(try lia).
   all: rewrite ?N.ltb_lt in *; ltac1:(try lia).
-  all: subst; rewrite N_modulo_10_spec in *; specialize N_modulo_le with (n := n) (m := 10%N) as ?; ltac1:(try lia).
+  all: subst; rewrite Nmod_10_spec in *; specialize N_modulo_le with (n := n) (m := 10%N) as ?; ltac1:(try lia).
 Qed.
 Time Compute to_funs [N2str_f_prog].
 
@@ -101,96 +101,96 @@ Proof.
 Qed.
 Time Compute to_funs [N2str_prog].
 
-Theorem list_length_equation: ltac2:(unfold_fix_type '@list_length).
-Proof. unfold_fix_proof '@list_length. Qed.
+Theorem list_len_equation: ltac2:(unfold_fix_type '@list_len).
+Proof. unfold_fix_proof '@list_len. Qed.
 
-Derive list_length_prog
-  in ltac2:(relcompile_tpe 'list_length_prog '@list_length [])
-  as list_length_prog_proof.
+Derive list_len_prog
+  in ltac2:(relcompile_tpe 'list_len_prog '@list_len [])
+  as list_len_prog_proof.
 Proof.
   time relcompile.
 Qed.
-Time Compute to_funs [list_length_prog].
+Time Compute to_funs [list_len_prog].
 
-Theorem list_append_equation: ltac2:(unfold_fix_type '@list_append).
-Proof. unfold_fix_proof '@list_append. Qed.
+Theorem list_app_equation: ltac2:(unfold_fix_type '@list_app).
+Proof. unfold_fix_proof '@list_app. Qed.
 
-Derive list_append_prog
-  in ltac2:(relcompile_tpe 'list_append_prog '@list_append [])
-  as list_append_prog_proof.
+Derive list_app_prog
+  in ltac2:(relcompile_tpe 'list_app_prog '@list_app [])
+  as list_app_prog_proof.
 Proof.
   time relcompile.
 Qed.
-Time Compute to_funs [list_append_prog].
+Time Compute to_funs [list_app_prog].
 
 Theorem flatten_equation: ltac2:(unfold_fix_type '@flatten).
 Proof. unfold_fix_proof '@flatten. Qed.
 
 Derive flatten_prog
-  in ltac2:(relcompile_tpe 'flatten_prog '@flatten ['@list_append])
+  in ltac2:(relcompile_tpe 'flatten_prog '@flatten ['@list_app])
   as flatten_prog_proof.
 Proof.
   time relcompile.
 Qed.
 Time Compute to_funs [flatten_prog].
 
-Theorem app_list_length_equation: ltac2:(unfold_fix_type '@app_list_length).
-Proof. unfold_fix_proof '@app_list_length. Qed.
+Theorem appl_len_equation: ltac2:(unfold_fix_type '@appl_len).
+Proof. unfold_fix_proof '@appl_len. Qed.
 
-Derive app_list_length_prog
-  in ltac2:(relcompile_tpe 'app_list_length_prog '@app_list_length ['@list_length])
-  as app_list_length_prog_proof.
+Derive appl_len_prog
+  in ltac2:(relcompile_tpe 'appl_len_prog '@appl_len ['@list_len])
+  as appl_len_prog_proof.
 Proof.
   time relcompile.
 Qed.
-Time Compute to_funs [app_list_length_prog].
+Time Compute to_funs [appl_len_prog].
 
-Derive mul_N_10_prog
-  in ltac2:(relcompile_tpe 'mul_N_10_prog 'mul_N_10 [])
-  as mul_N_10_prog_proof.
+Derive mulN_10_prog
+  in ltac2:(relcompile_tpe 'mulN_10_prog 'mulN_10 [])
+  as mulN_10_prog_proof.
 Proof.
   time relcompile.
 Qed.
-Time Compute to_funs [mul_N_10_prog].
+Time Compute to_funs [mulN_10_prog].
 
-Derive mul_N_256_prog
-  in ltac2:(relcompile_tpe 'mul_N_256_prog 'mul_N_256 [])
-  as mul_N_256_prog_proof.
+Derive mulN_256_prog
+  in ltac2:(relcompile_tpe 'mulN_256_prog 'mulN_256 [])
+  as mulN_256_prog_proof.
 Proof.
   time relcompile.
 Qed.
-Time Compute to_funs [mul_N_256_prog].
+Time Compute to_funs [mulN_256_prog].
 
-Derive mul_nat_8_prog
-  in ltac2:(relcompile_tpe 'mul_nat_8_prog 'mul_nat_8 [])
-  as mul_nat_8_prog_proof.
+Derive mulnat_8_prog
+  in ltac2:(relcompile_tpe 'mulnat_8_prog 'mulnat_8 [])
+  as mulnat_8_prog_proof.
 Proof.
   time relcompile.
 Qed.
-Time Compute to_funs [mul_nat_8_prog].
+Time Compute to_funs [mulnat_8_prog].
 
-Derive mul_nat_10_prog
-  in ltac2:(relcompile_tpe 'mul_nat_10_prog 'mul_nat_10 [])
-  as mul_nat_10_prog_proof.
+Derive mulnat10_prog
+  in ltac2:(relcompile_tpe 'mulnat10_prog 'mulnat10 [])
+  as mulnat10_prog_proof.
 Proof.
   time relcompile.
 Qed.
-Time Compute to_funs [mul_nat_10_prog].
+Time Compute to_funs [mulnat10_prog].
 
-Theorem N2ascii_f_equation: ltac2:(unfold_fix_type '@N2ascii_f).
-Proof. unfold_fix_proof '@N2ascii_f. Qed.
-Derive N2ascii_f_prog
-  in ltac2:(relcompile_tpe 'N2ascii_f_prog 'N2ascii_f ['N_modulo_256; 'string_append])
-  as N2ascii_f_prog_proof.
+Theorem N2asciif_equation: ltac2:(unfold_fix_type '@N2asciif).
+Proof. unfold_fix_proof '@N2asciif. Qed.
+Derive N2asciif_prog
+  in ltac2:(relcompile_tpe 'N2asciif_prog 'N2asciif ['Nmod_256; 'str_app])
+  as N2asciif_prog_proof.
 Proof.
   time relcompile.
   all: ltac1:(try lia).
-  all: subst; rewrite N_modulo_256_spec in *; specialize N_modulo_lt with (n := n) (m := 256%N) as ?; ltac1:(try lia).
+  all: subst; rewrite Nmod_256_spec in *; specialize N_modulo_lt with (n := n) (m := 256%N) as ?; ltac1:(try lia).
 Qed.
-Time Compute to_funs [N2ascii_f_prog].
+Time Compute to_funs [N2asciif_prog].
 
 Derive N2ascii_prog
-  in ltac2:(relcompile_tpe 'N2ascii_prog 'N2ascii ['N2ascii_f])
+  in ltac2:(relcompile_tpe 'N2ascii_prog 'N2ascii ['N2asciif])
   as N2ascii_prog_proof.
 Proof.
   time relcompile.
@@ -198,34 +198,34 @@ Proof.
 Qed.
 Time Compute to_funs [N2ascii_prog].
 
-Derive N2ascii_default_prog
-  in ltac2:(relcompile_tpe 'N2ascii_default_prog 'N2ascii_default ['N2ascii])
-  as N2ascii_default_prog_proof.
+Derive N2asciid_prog
+  in ltac2:(relcompile_tpe 'N2asciid_prog 'N2asciid ['N2ascii])
+  as N2asciid_prog_proof.
 Proof.
   time relcompile.
 Qed.
-Time Compute to_funs [N2ascii_default_prog].
+Time Compute to_funs [N2asciid_prog].
 
 Definition CompilerUtils_funs := [
-  mul_nat_8_prog;
-  mul_nat_10_prog;
-  mul_N_10_prog;
-  mul_N_256_prog;
-  nat_modulo_10_prog;
-  N_modulo_10_prog;
-  N_modulo_256_prog;
-  num2str_f_prog;
+  mulnat_8_prog;
+  mulnat10_prog;
+  mulN_10_prog;
+  mulN_256_prog;
+  natmod10_prog;
+  Nmod_10_prog;
+  Nmod_256_prog;
+  num2strf_prog;
   num2str_prog;
   N2str_f_prog;
   N2str_prog;
-  list_length_prog;
-  list_append_prog;
+  list_len_prog;
+  list_app_prog;
   flatten_prog;
-  app_list_length_prog;
-  string_append_prog;
-  N2ascii_f_prog;
+  appl_len_prog;
+  str_app_prog;
+  N2asciif_prog;
   N2ascii_prog;
-  N2ascii_default_prog
+  N2asciid_prog
 ].
 
 Ltac2 assert_eval_app (fname: constr) :=
@@ -244,22 +244,22 @@ Ltac2 assert_eval_app_by (fname: constr) (prf: constr) (list_constr_hyp: constr)
   ).
 
 Ltac2 assert_eval_app_compiler_utils (hlookup_constr: constr) :=
-  assert_eval_app_by 'mul_nat_8 'mul_nat_8_prog_proof hlookup_constr 0;
-  assert_eval_app_by 'mul_nat_10 'mul_nat_10_prog_proof hlookup_constr 1;
-  assert_eval_app_by 'mul_N_10 'mul_N_10_prog_proof hlookup_constr 2;
-  assert_eval_app_by 'mul_N_256 'mul_N_256_prog_proof hlookup_constr 3;
-  assert_eval_app_by 'nat_modulo_10 'nat_modulo_10_prog_proof hlookup_constr 4;
-  assert_eval_app_by 'N_modulo_10 'N_modulo_10_prog_proof hlookup_constr 5;
-  assert_eval_app_by 'N_modulo_256 'N_modulo_256_prog_proof hlookup_constr 6;
-  assert_eval_app_by 'num2str_f 'num2str_f_prog_proof hlookup_constr 7;
+  assert_eval_app_by 'mulnat_8 'mulnat_8_prog_proof hlookup_constr 0;
+  assert_eval_app_by 'mulnat10 'mulnat10_prog_proof hlookup_constr 1;
+  assert_eval_app_by 'mulN_10 'mulN_10_prog_proof hlookup_constr 2;
+  assert_eval_app_by 'mulN_256 'mulN_256_prog_proof hlookup_constr 3;
+  assert_eval_app_by 'natmod10 'natmod10_prog_proof hlookup_constr 4;
+  assert_eval_app_by 'Nmod_10 'Nmod_10_prog_proof hlookup_constr 5;
+  assert_eval_app_by 'Nmod_256 'Nmod_256_prog_proof hlookup_constr 6;
+  assert_eval_app_by 'num2strf 'num2strf_prog_proof hlookup_constr 7;
   assert_eval_app_by 'num2str 'num2str_prog_proof hlookup_constr 8;
   assert_eval_app_by 'N2str_f 'N2str_f_prog_proof hlookup_constr 9;
   assert_eval_app_by 'N2str 'N2str_prog_proof hlookup_constr 10;
-  assert_eval_app_by '@list_length 'list_length_prog_proof hlookup_constr 11;
-  assert_eval_app_by '@list_append 'list_append_prog_proof hlookup_constr 12;
+  assert_eval_app_by '@list_len 'list_len_prog_proof hlookup_constr 11;
+  assert_eval_app_by '@list_app 'list_app_prog_proof hlookup_constr 12;
   assert_eval_app_by '@flatten 'flatten_prog_proof hlookup_constr 13;
-  assert_eval_app_by '@app_list_length 'app_list_length_prog_proof hlookup_constr 14;
-  assert_eval_app_by 'string_append 'string_append_prog_proof hlookup_constr 15;
-  assert_eval_app_by 'N2ascii_f 'N2ascii_f_prog_proof hlookup_constr 16;
+  assert_eval_app_by '@appl_len 'appl_len_prog_proof hlookup_constr 14;
+  assert_eval_app_by 'str_app 'str_app_prog_proof hlookup_constr 15;
+  assert_eval_app_by 'N2asciif 'N2asciif_prog_proof hlookup_constr 16;
   assert_eval_app_by 'N2ascii 'N2ascii_prog_proof hlookup_constr 17;
-  assert_eval_app_by 'N2ascii_default 'N2ascii_default_prog_proof hlookup_constr 18.
+  assert_eval_app_by 'N2asciid 'N2asciid_prog_proof hlookup_constr 18.
