coq/theories/imperative/SomeProgram.v
@@ -17,14 +17,21 @@ Definition some_program1 :=
       Seq (
         PutChar (Const (word.of_Z 65))
       ) (
-        Return (Const (word.of_Z 0))
+        Seq
+          (Assign (name_enc "x") (Const (word.of_Z 42)))
+          (Seq
+            (If (Test Equal (Var (name_enc "x")) (Const (word.of_Z 42)))
+                (PutChar (Const (word.of_Z 66)))
+                (PutChar (Const (word.of_Z 67)))
+            )
+          (Return (Const (word.of_Z 0))))
       )
     )
   ].
 
 Eval lazy in imp2str some_program1.
 
-Eval lazy in str2imp (list_ascii_of_string (imp2str some_program1)).
+Eval lazy in imp2str (str2imp (list_ascii_of_string (imp2str some_program1))).
 
 Eval lazy in codegen some_program1.
 
