coq/theories/parsing/ExtractParser.v
@@ -1,0 +1,55 @@
+Set Warnings "-notation-overridden,-notation-incompatible-prefix".
+From Stdlib Require Extraction.
+Set Extraction Output Directory "./extraction".
+Extraction Language OCaml.
+From Stdlib Require Import ExtrOcamlBasic.
+From Stdlib Require Import ExtrOcamlString.
+
+From impboot.utils Require Import Core.
+From impboot.parsing Require Import Parser.
+From impboot.imperative Require Import Printing.
+
+Extract Inductive nat => "int64"
+  [ "0L" "(fun x -> Int64.add x 1L)" ]
+  "(fun zero succ n -> if Int64.equal n 0L then zero () else succ (Int64.sub n 1L))".
+
+Extract Inductive positive => "int64"
+[ "(fun p -> Int64.add 1L (Int64.mul 2L p))" "(fun p -> Int64.mul 2L p)" "1L" ]
+"(fun f2p1 f2p f1 p ->
+  if Int64.compare p 1L <= 0 then f1 () else if Int64.equal (Int64.rem p 2L) 0L then f2p (Int64.div p 2L) else f2p1 (Int64.div p 2L))".
+
+Extract Inductive N => "int64" [ "0L" "" ]
+  "(fun f0 fp n -> if Int64.equal n 0L then f0 () else fp n)".
+
+Extract Inlined Constant Nat.add => "Int64.add".
+Extract Inlined Constant Nat.mul => "Int64.mul".
+Extract Inlined Constant Nat.eqb => "Int64.sub".
+
+Extract Inlined Constant Pos.add => "Int64.add".
+Extract Inlined Constant Pos.succ => "Int64.succ".
+Extract Inlined Constant Pos.pred => "fun n -> Int64.max 1L (Int64.sub n 1L)".
+Extract Inlined Constant Pos.sub => "fun n m -> Int64.max 1L (Int64.sub n m)".
+Extract Inlined Constant Pos.mul => "Int64.mul".
+Extract Inlined Constant Pos.min => "Int64.min".
+Extract Inlined Constant Pos.max => "Int64.max".
+Extract Inlined Constant Pos.compare =>
+ "fun x y -> if Int64.equal x y then Eq else if Int64.compare x y < 0 then Lt else Gt".
+Extract Inlined Constant Pos.compare_cont =>
+ "fun c x y -> if Int64.equal x y then c else if Int64.compare x y < 0 then Lt else Gt".
+
+Extract Inlined Constant N.add => "Int64.add".
+Extract Inlined Constant N.succ => "Int64.succ".
+Extract Inlined Constant N.pred => "(fun n -> Int64.max 0L (Int64.sub n 1L))".
+Extract Inlined Constant N.sub => "(fun n m -> Int64.max 0L (Int64.sub n m))".
+Extract Inlined Constant N.mul => "Int64.mul".
+Extract Inlined Constant N.min => "Int64.min".
+Extract Inlined Constant N.max => "Int64.max".
+Extract Inlined Constant N.div => "(fun a b -> if Int64.equal b 0L then 0L else Int64.div a b)".
+Extract Inlined Constant N.modulo => "(fun a b -> if Int64.equal b 0L then a else Int64.rem a b)".
+Extract Constant N.compare =>
+ "fun x y -> if Int64.equal x y then Eq else if Int64.compare x y < 0 then Lt else Gt".
+Extract Constant N.leb => "(fun n m -> Int64.compare n m <= 0)".
+Extract Constant N.to_nat => "(fun x -> x)".
+
+
+Extraction "ExtractParser.ml" str2imp imp2str.
