coq/theories/parsing/ParserProofs.v
@@ -1,4 +1,4 @@
-(* Require Import impboot.utils.Core.
+Require Import impboot.utils.Core.
 Require Import impboot.parsing.Parser.
 Require Import impboot.imp2asm.ImpToASMCodegenProofs.
 Require Import Patat.Patat.
@@ -9,18 +9,34 @@ Ltac cleanup :=
   | H: (_, _) = (_, _) |- _ => inversion H; clear H; subst
   end.
 
-Theorem read_num_length: ∀l h xs n ys f acc x,
-  read_num l h f x acc xs = (n, ys) ->
+Theorem read_nmc_length: ∀ xs n ys acc,
+  read_nmc acc xs = (n, ys) ->
     List.length ys ≤ List.length xs ∧ (xs ≠ ys -> List.length ys < List.length xs)%nat.
 Proof.
   induction xs; intros; simpl in *; unfold dlet in *; cleanup; simpl.
   1: split; eauto; intros; congruence.
   destruct (_ <? _)%N eqn:?; simpl in *; cleanup; simpl in *.
   1: split; [lia|]; intros; congruence.
-  destruct (N_of_ascii h<? _)%N eqn:?; simpl in *; cleanup; simpl in *.
+  destruct (_ <? N_of_ascii _)%N eqn:?; simpl in *; cleanup; simpl in *.
   1: split; [lia|]; intros; congruence.
-  pat `read_num _ _ _ _ _ _ = _` at rename pat into Hread_num.
-  pat `forall n ys f acc x, _` at eapply pat in Hread_num.
+  pat `read_nmc _ _ = _` at rename pat into Hread_num.
+  pat `forall n ys acc, _` at eapply pat in Hread_num.
+  split; [lia|].
+  intros; lia.
+Qed.
+
+Theorem read_alp_length: ∀ xs n ys acc,
+  read_alp acc xs = (n, ys) ->
+    List.length ys ≤ List.length xs ∧ (xs ≠ ys -> List.length ys < List.length xs)%nat.
+Proof.
+  induction xs; intros; simpl in *; unfold dlet in *; cleanup; simpl.
+  1: split; eauto; intros; congruence.
+  destruct (_ <? _)%N eqn:?; simpl in *; cleanup; simpl in *.
+  1: split; [lia|]; intros; congruence.
+  destruct (_ <? N_of_ascii _)%N eqn:?; simpl in *; cleanup; simpl in *.
+  1: split; [lia|]; intros; congruence.
+  pat `read_alp _ _ = _` at rename pat into Hread_num.
+  pat `forall n ys acc, _` at eapply pat in Hread_num.
   split; [lia|].
   intros; lia.
 Qed.
@@ -45,27 +61,34 @@ Proof.
     eapply IHfuel
   | |- (let (_, _) := if ?c then _ else _ in _) <> _ =>
     destruct c eqn:?
-  | |- (let (_, _) := read_num _ _ _ _ _ cs in _) <> _ =>
-    destruct read_num eqn:?
-  | H: _ = _ :: ?l |- (let (_, _) := read_num ?a1 ?a2 ?a3 ?a4 ?a5 ?l in _) <> _ =>
-    destruct (read_num a1 a2 a3 a4 a5 l) eqn:?
+  | |- (let (_, _) := read_nmc _ cs in _) <> _ =>
+    destruct read_nmc eqn:?
+  | |- (let (_, _) := read_alp _ cs in _) <> _ =>
+    destruct read_alp eqn:?
+  | H: _ = _ :: ?l |- (let (_, _) := read_nmc ?a1 ?l in _) <> _ =>
+    destruct (read_nmc a1 l) eqn:?
+  | H: _ = _ :: ?l |- (let (_, _) := read_alp ?a1 ?l in _) <> _ =>
+    destruct (read_alp a1 l) eqn:?
   | |- (List.length (end_line _) <= _)%nat =>
     eapply Nat.le_trans; [eapply end_line_length|]; lia
   | H: (S _ <= S _)%nat |- _ =>
     eapply le_S_n in H
   | H: cs = ?h :: ?t |- (List.length (?h :: ?t) <= _)%nat =>
     rewrite negb_true_iff, Nat.eqb_neq in *; simpl in *; congruence
-  | H: read_num _ _ _ _ _ ?t = (_, _) |- _ =>
-    eapply read_num_length in H
-  | H: context C [CompilerUtils.list_length _] |- _ =>
-    rewrite list_length_spec in H; simpl in H
+  | H: read_nmc _ ?t = (_, _) |- _ =>
+    eapply read_nmc_length in H
+  | H: read_alp _ ?t = (_, _) |- _ =>
+    eapply read_alp_length in H
+  | H: context C [CompilerUtils.list_len _] |- _ =>
+    rewrite list_len_spec in H; simpl in H
   | H: (_ =? _)%nat = false |- _ =>
     rewrite Nat.eqb_neq in H
   | _ =>
     progress unfold dlet in *
-  | |- List.length (_ :: _) <= _ => progress simpl
+  | |- List.length (_ :: _) <= _ => progress simpl in *
   | _ => lia
   end.
+  all: simpl in *; lia.
 Qed.
 
 Theorem lexer_terminates: forall (inp: string),
@@ -73,6 +96,6 @@ Theorem lexer_terminates: forall (inp: string),
 Proof.
   intros; unfold lexer_i, dlet.
   eapply lex_terminates.
-  rewrite list_length_spec; simpl.
+  rewrite list_len_spec; simpl.
   eapply Nat.le_refl.
-Qed. *)
+Qed.
